Prove rewrite-rule-independent parts of rewrite Wf
We still need to prove things about the individual rewrite rules

After     | File Name                                          | Before    || Change     | % Change
-----------------------------------------------------------------------------------------------------
23m03.10s | Total                                              | 11m59.51s || +11m03.58s | +92.22%
-----------------------------------------------------------------------------------------------------
10m56.17s | Experiments/NewPipeline/RewriterProofs             | 0m01.32s  || +10m54.84s | +49609.84%
5m53.88s  | Experiments/NewPipeline/SlowPrimeSynthesisExamples | 5m49.62s  || +0m04.25s  | +1.21%
1m37.55s  | Experiments/NewPipeline/Toplevel2                  | 1m33.45s  || +0m04.09s  | +4.38%
4m31.67s  | Experiments/NewPipeline/Toplevel1                  | 4m31.39s  || +0m00.28s  | +0.10%
0m01.45s  | Experiments/NewPipeline/CLI                        | 0m01.34s  || +0m00.10s  | +8.20%
0m01.24s  | Experiments/NewPipeline/StandaloneOCamlMain        | 0m01.25s  || -0m00.01s  | -0.80%
0m01.14s  | Experiments/NewPipeline/StandaloneHaskellMain      | 0m01.15s  || -0m00.01s  | -0.86%

src/Experiments/NewPipeline/RewriterProofs.v
@@ -1,4 +1,5 @@
 Require Import Coq.ZArith.ZArith.
+Require Import Coq.micromega.Lia.
 Require Import Coq.Lists.List.
 Require Import Coq.Classes.Morphisms.
 Require Import Coq.MSets.MSetPositive.
@@ -6,20 +7,31 @@ Require Import Coq.FSets.FMapPositive.
 Require Import Crypto.Experiments.NewPipeline.Language.
 Require Import Crypto.Experiments.NewPipeline.LanguageInversion.
 Require Import Crypto.Experiments.NewPipeline.LanguageWf.
+Require Import Crypto.Experiments.NewPipeline.UnderLetsProofs.
+Require Import Crypto.Experiments.NewPipeline.GENERATEDIdentifiersWithoutTypesProofs.
 Require Import Crypto.Experiments.NewPipeline.Rewriter.
 Require Import Crypto.Util.Tactics.BreakMatch.
 Require Import Crypto.Util.Tactics.SplitInContext.
 Require Import Crypto.Util.Tactics.SpecializeAllWays.
+Require Import Crypto.Util.Tactics.SpecializeBy.
 Require Import Crypto.Util.Tactics.RewriteHyp.
+Require Import Crypto.Util.Tactics.Head.
 Require Import Crypto.Util.Prod.
 Require Import Crypto.Util.ListUtil.
+Require Import Crypto.Util.Option.
+Require Import Crypto.Util.CPSNotations.
+Require Import Crypto.Util.HProp.
+Require Import Crypto.Util.Decidable.
 Import ListNotations. Local Open Scope list_scope.
 Local Open Scope Z_scope.
 
+Import EqNotations.
 Module Compilers.
   Import Language.Compilers.
   Import LanguageInversion.Compilers.
   Import LanguageWf.Compilers.
+  Import UnderLetsProofs.Compilers.
+  Import GENERATEDIdentifiersWithoutTypesProofs.Compilers.
   Import Rewriter.Compilers.
   Import expr.Notations.
   Import defaults.
@@ -27,71 +39,1335 @@ Module Compilers.
   Module Import RewriteRules.
     Import Rewriter.Compilers.RewriteRules.
 
-    (*
     Module Compile.
       Import Rewriter.Compilers.RewriteRules.Compile.
 
-      Section with_var0.
-        Context {base_type} {ident var : type.type base_type -> Type}.
+      Section with_type0.
+        Context {base_type} {ident : type.type base_type -> Type}.
         Local Notation type := (type.type base_type).
-        Local Notation expr := (@expr.expr base_type ident var).
-        Local Notation UnderLets := (@UnderLets.UnderLets base_type ident var).
+        Local Notation expr := (@expr.expr base_type ident).
+        Local Notation UnderLets := (@UnderLets.UnderLets base_type ident).
         Let type_base (t : base_type) : type := type.base t.
         Coercion type_base : base_type >-> type.
-      End with_var0.
 
-      Section full.
-        Context {var : type.type base.type -> Type}.
-        Local Notation expr := (@expr base.type ident).
-        Local Notation value := (@Compile.value base.type ident var).
-        Local Notation value_with_lets := (@Compile.value_with_lets base.type ident var).
-        Local Notation UnderLets := (UnderLets.UnderLets base.type ident var).
-        Local Notation reify_and_let_binds_cps := (@Compile.reify_and_let_binds_cps ident var (@UnderLets.reify_and_let_binds_base_cps var)).
-        Local Notation reflect := (@Compile.reflect ident var).
-        (*
+        Section with_var2.
+          Context {var1 var2 : type -> Type}.
+
+          Local Notation value'1 := (@value' base_type ident var1).
+          Local Notation value'2 := (@value' base_type ident var2).
+          Local Notation value1 := (@value base_type ident var1).
+          Local Notation value2 := (@value base_type ident var2).
+          Local Notation value_with_lets1 := (@value_with_lets base_type ident var1).
+          Local Notation value_with_lets2 := (@value_with_lets base_type ident var2).
+          Local Notation Base_value := (@Base_value base_type ident).
+          Local Notation splice_under_lets_with_value := (@splice_under_lets_with_value base_type ident).
+          Local Notation splice_value_with_lets := (@splice_value_with_lets base_type ident).
+
+          Fixpoint wf_value' {with_lets : bool} G {t : type} : value'1 with_lets t -> value'2 with_lets t -> Prop
+            := match t, with_lets with
+               | type.base t, true => UnderLets.wf (fun G' => expr.wf G') G
+               | type.base t, false => expr.wf G
+               | type.arrow s d, _
+                 => fun f1 f2
+                    => (forall seg G' v1 v2,
+                           G' = (seg ++ G)%list
+                           -> @wf_value' false seg s v1 v2
+                           -> @wf_value' true G' d (f1 v1) (f2 v2))
+               end.
+
+          Definition wf_value G {t} : value1 t -> value2 t -> Prop := @wf_value' false G t.
+          Definition wf_value_with_lets G {t} : value_with_lets1 t -> value_with_lets2 t -> Prop := @wf_value' true G t.
+
+          Lemma wf_value'_Proper_list {with_lets} G1 G2
+                (HG1G2 : forall t v1 v2, List.In (existT _ t (v1, v2)) G1 -> List.In (existT _ t (v1, v2)) G2)
+                t e1 e2
+                (Hwf : @wf_value' with_lets G1 t e1 e2)
+            : @wf_value' with_lets G2 t e1 e2.
+          Proof.
+            revert Hwf; revert dependent with_lets; revert dependent G2; revert dependent G1; induction t;
+              repeat first [ progress cbn in *
+                           | progress intros
+                           | solve [ eauto ]
+                           | progress subst
+                           | progress destruct_head'_or
+                           | progress inversion_sigma
+                           | progress inversion_prod
+                           | progress break_innermost_match_hyps
+                           | eapply UnderLets.wf_Proper_list; [ .. | solve [ eauto ] ]
+                           | wf_unsafe_t_step
+                           | match goal with H : _ |- _ => solve [ eapply H; [ .. | solve [ eauto ] ]; wf_t ] end ].
+          Qed.
+
+          Lemma wf_Base_value G {t} v1 v2 (Hwf : @wf_value G t v1 v2)
+            : @wf_value_with_lets G t (Base_value v1) (Base_value v2).
+          Proof.
+            destruct t; cbn; intros; subst; hnf; try constructor; try assumption.
+            eapply wf_value'_Proper_list; [ | solve [ eauto ] ]; trivial.
+          Qed.
+
+          Lemma wf_splice_under_lets_with_value {T1 T2 t}
+                G
+                (x1 : @UnderLets var1 T1) (x2 : @UnderLets var2 T2)
+                (e1 : T1 -> value_with_lets1 t) (e2 : T2 -> value_with_lets2 t)
+                (Hx : UnderLets.wf (fun G' a1 a2 => wf_value_with_lets G' (e1 a1) (e2 a2)) G x1 x2)
+            : wf_value_with_lets G (splice_under_lets_with_value x1 e1) (splice_under_lets_with_value x2 e2).
+          Proof.
+            cbv [wf_value_with_lets] in *.
+            revert dependent G; induction t as [t|s IHs d IHd]; cbn [splice_under_lets_with_value wf_value']; intros.
+            { eapply UnderLets.wf_splice; eauto. }
+            { intros; subst; apply IHd.
+              eapply UnderLets.wf_Proper_list_impl; [ | | solve [ eauto ] ]; wf_t.
+              eapply wf_value'_Proper_list; [ | solve [ eauto ] ]; wf_t. }
+          Qed.
+
+          Lemma wf_splice_value_with_lets {t t'}
+                G
+                (x1 : value_with_lets1 t) (x2 : value_with_lets2 t)
+                (e1 : value1 t -> value_with_lets1 t') (e2 : value2 t -> value_with_lets2 t')
+                (Hx : wf_value_with_lets G x1 x2)
+                (He : forall seg G' v1 v2, (G' = (seg ++ G)%list) -> wf_value G' v1 v2 -> wf_value_with_lets G' (e1 v1) (e2 v2))
+            : wf_value_with_lets G (splice_value_with_lets x1 e1) (splice_value_with_lets x2 e2).
+          Proof.
+            destruct t; cbn [splice_value_with_lets].
+            { eapply wf_splice_under_lets_with_value.
+              eapply UnderLets.wf_Proper_list_impl; [ | | eassumption ]; trivial; wf_t. }
+            { eapply wf_value'_Proper_list; [ | eapply He with (seg:=nil); hnf in Hx |- * ].
+              { eauto; subst G'; wf_t. }
+              { reflexivity. }
+              { intros; subst; eapply wf_value'_Proper_list; [ | solve [ eauto ] ]; wf_t. } }
+          Qed.
+
+          Section wf.
+            Context (G : list { t : _ & var1 t * var2 t }%type).
+            Inductive wf_anyexpr : forall t, @AnyExpr.anyexpr base_type ident var1 -> @AnyExpr.anyexpr base_type ident var2 -> Prop :=
+            | Wf_wrap {t : base_type} {e1 e2} : expr.wf (t:=t) G e1 e2 -> @wf_anyexpr (type.base t) (AnyExpr.wrap e1) (AnyExpr.wrap e2).
+          End wf.
+        End with_var2.
+      End with_type0.
+      Import AnyExpr.
+      Section with_type.
+        Context {ident : type.type base.type -> Type}
+                {pident : Type}
+                (full_types : pident -> Type)
+                (invert_bind_args : forall t (idc : ident t) (pidc : pident), option (full_types pidc))
+                (type_of_pident : forall (pidc : pident), full_types pidc -> type.type base.type)
+                (pident_to_typed : forall (pidc : pident) (args : full_types pidc), ident (type_of_pident pidc args))
+                (eta_ident_cps : forall {T : type.type base.type -> Type} {t} (idc : ident t)
+                                        (f : forall t', ident t' -> T t'),
+                    T t)
+                (eta_ident_cps_correct : forall T t idc f, @eta_ident_cps T t idc f = f _ idc)
+                (of_typed_ident : forall {t}, ident t -> pident)
+                (arg_types : pident -> option Type)
+                (bind_args : forall {t} (idc : ident t), match arg_types (of_typed_ident idc) return Type with Some t => t | None => unit end)
+                (pident_beq : pident -> pident -> bool)
+                (try_make_transport_ident_cps : forall (P : pident -> Type) (idc1 idc2 : pident), ~> option (P idc1 -> P idc2))
+                (pident_to_typed_invert_bind_args_type
+                 : forall t idc p f, invert_bind_args t idc p = Some f -> t = type_of_pident p f)
+                (pident_to_typed_invert_bind_args
+                 : forall t idc p f (pf : invert_bind_args t idc p = Some f),
+                    pident_to_typed p f = rew [ident] pident_to_typed_invert_bind_args_type t idc p f pf in idc)
+                (pident_bl : forall p q, pident_beq p q = true -> p = q)
+                (pident_lb : forall p q, p = q -> pident_beq p q = true)
+                (try_make_transport_ident_cps_correct
+                 : forall P idc1 idc2 T k,
+                    try_make_transport_ident_cps P idc1 idc2 T k
+                    = k (match Sumbool.sumbool_of_bool (pident_beq idc1 idc2) with
+                         | left pf => Some (fun v => rew [P] pident_bl _ _ pf in v)
+                         | right _ => None
+                         end)).
+        Local Notation type := (type.type base.type).
+        Local Notation pattern := (@pattern.pattern pident).
+        Local Notation expr := (@expr.expr base.type ident).
+        Local Notation anyexpr := (@anyexpr base.type ident).
+        Local Notation UnderLets := (@UnderLets.UnderLets base.type ident).
+        Local Notation ptype := (type.type pattern.base.type).
+        Local Notation value' := (@value' base.type ident).
+        Local Notation value := (@value base.type ident).
+        Local Notation value_with_lets := (@value_with_lets base.type ident).
+        Local Notation Base_value := (@Base_value base.type ident).
+        Local Notation splice_under_lets_with_value := (@splice_under_lets_with_value base.type ident).
+        Local Notation splice_value_with_lets := (@splice_value_with_lets base.type ident).
+        Local Notation reify := (@reify ident).
+        Local Notation reflect := (@reflect ident).
+        Local Notation rawexpr := (@rawexpr ident).
+        Local Notation eval_decision_tree var := (@eval_decision_tree ident var pident full_types invert_bind_args type_of_pident pident_to_typed).
+        Local Notation reveal_rawexpr e := (@reveal_rawexpr_cps ident _ e _ id).
+        Local Notation bind_data_cps var := (@bind_data_cps ident var pident of_typed_ident arg_types bind_args try_make_transport_ident_cps).
+        Local Notation bind_data e p := (@bind_data_cps _ e p _ id).
+        Local Notation ptype_interp := (@ptype_interp ident).
+        Local Notation binding_dataT var := (@binding_dataT ident var pident arg_types).
+
+        Section with_var2.
+          Context {var1 var2 : type -> Type}.
+
+          Context (reify_and_let_binds_base_cps1 : forall (t : base.type), @expr var1 t -> forall T, (@expr var1 t -> @UnderLets var1 T) -> @UnderLets var1 T)
+                  (reify_and_let_binds_base_cps2 : forall (t : base.type), @expr var2 t -> forall T, (@expr var2 t -> @UnderLets var2 T) -> @UnderLets var2 T)
+                  (wf_reify_and_let_binds_base_cps
+                   : forall G (t : base.type) x1 x2 T1 T2 P
+                            (Hx : expr.wf G x1 x2)
+                            (e1 : expr t -> @UnderLets var1 T1) (e2 : expr t -> @UnderLets var2 T2)
+                            (He : forall x1 x2 G' seg, (G' = (seg ++ G)%list) -> expr.wf G' x1 x2 -> UnderLets.wf P G' (e1 x1) (e2 x2)),
+                      UnderLets.wf P G (reify_and_let_binds_base_cps1 t x1 T1 e1) (reify_and_let_binds_base_cps2 t x2 T2 e2)).
+
+          Local Notation wf_value' := (@wf_value' base.type ident var1 var2).
+          Local Notation wf_value := (@wf_value base.type ident var1 var2).
+          Local Notation wf_value_with_lets := (@wf_value_with_lets base.type ident var1 var2).
+          Local Notation reify_and_let_binds_cps1 := (@reify_and_let_binds_cps ident var1 reify_and_let_binds_base_cps1).
+          Local Notation reify_and_let_binds_cps2 := (@reify_and_let_binds_cps ident var2 reify_and_let_binds_base_cps2).
+          Local Notation rewrite_rulesT1 := (@rewrite_rulesT ident var1 pident arg_types).
+          Local Notation rewrite_rulesT2 := (@rewrite_rulesT ident var2 pident arg_types).
+          Local Notation eval_rewrite_rules1 := (@eval_rewrite_rules ident var1 pident full_types invert_bind_args type_of_pident pident_to_typed of_typed_ident arg_types bind_args try_make_transport_ident_cps).
+          Local Notation eval_rewrite_rules2 := (@eval_rewrite_rules ident var2 pident full_types invert_bind_args type_of_pident pident_to_typed of_typed_ident arg_types bind_args try_make_transport_ident_cps).
+
+          Fixpoint wf_reify {with_lets} G {t}
+            : forall e1 e2, @wf_value' with_lets G t e1 e2 -> expr.wf G (@reify _ with_lets t e1) (@reify _ with_lets t e2)
+          with wf_reflect {with_lets} G {t}
+               : forall e1 e2, expr.wf G e1 e2 -> @wf_value' with_lets G t (@reflect _ with_lets t e1) (@reflect _ with_lets t e2).
+          Proof using Type.
+            { destruct t as [t|s d];
+                [ clear wf_reflect wf_reify
+                | specialize (fun with_lets G => @wf_reify with_lets G d); specialize (fun with_lets G => wf_reflect with_lets G s) ].
+              { destruct with_lets; cbn; intros; auto using UnderLets.wf_to_expr. }
+              { intros e1 e2 Hwf.
+                change (reify e1) with (λ x, @reify _ _ d (e1 (@reflect _ _ s ($x))))%expr.
+                change (reify e2) with (λ x, @reify _ _ d (e2 (@reflect _ _ s ($x))))%expr.
+                constructor; intros; eapply wf_reify, Hwf with (seg:=cons _ nil); [ | eapply wf_reflect; constructor ]; wf_t. } }
+            { destruct t as [t|s d];
+                [ clear wf_reflect wf_reify
+                | specialize (fun with_lets G => @wf_reify with_lets G s); specialize (fun with_lets G => wf_reflect with_lets G d) ].
+              { destruct with_lets; repeat constructor; auto. }
+              { intros e1 e2 Hwf.
+                change (reflect e1) with (fun x => @reflect _ true d (e1 @ (@reify _ false s x)))%expr.
+                change (reflect e2) with (fun x => @reflect _ true d (e2 @ (@reify _ false s x)))%expr.
+                hnf; intros; subst.
+                eapply wf_reflect; constructor; [ wf_t | ].
+                eapply wf_reify, wf_value'_Proper_list; [ | eassumption ]; wf_t. } }
+          Qed.
+
+          Lemma wf_reify_and_let_binds_cps {with_lets} G {t} x1 x2
+                (Hx : @wf_value' with_lets G t x1 x2)
+                T1 T2 P
+                (e1 : expr t -> @UnderLets var1 T1) (e2 : expr t -> @UnderLets var2 T2)
+                (He : forall x1 x2 G' seg, (G' = (seg ++ G)%list) -> expr.wf G' x1 x2 -> UnderLets.wf P G' (e1 x1) (e2 x2))
+            : UnderLets.wf P G (@reify_and_let_binds_cps1 with_lets t x1 T1 e1) (@reify_and_let_binds_cps2 with_lets t x2 T2 e2).
+          Proof.
+            destruct t; [ destruct with_lets | ]; cbn [reify_and_let_binds_cps]; auto.
+            { eapply UnderLets.wf_splice; [ eapply Hx | ]; wf_t; destruct_head'_ex; wf_t.
+              eapply wf_reify_and_let_binds_base_cps; wf_t.
+              eapply He; rewrite app_assoc; wf_t. }
+            { eapply He with (seg:=nil); [ reflexivity | ].
+              eapply wf_reify; auto. }
+          Qed.
+
+          Inductive wf_rawexpr : list { t : type & var1 t * var2 t }%type -> forall {t}, @rawexpr var1 -> @expr var1 t -> @rawexpr var2 -> @expr var2 t -> Prop :=
+          | Wf_rIdent {t} G (idc : ident t) : wf_rawexpr G (rIdent idc (expr.Ident idc)) (expr.Ident idc) (rIdent idc (expr.Ident idc)) (expr.Ident idc)
+          | Wf_rApp {s d} G
+                    f1 (f1e : @expr var1 (s -> d)) x1 (x1e : @expr var1 s)
+                    f2 (f2e : @expr var2 (s -> d)) x2 (x2e : @expr var2 s)
+            : wf_rawexpr G f1 f1e f2 f2e
+              -> wf_rawexpr G x1 x1e x2 x2e
+              -> wf_rawexpr G
+                            (rApp f1 x1 (expr.App f1e x1e)) (expr.App f1e x1e)
+                            (rApp f2 x2 (expr.App f2e x2e)) (expr.App f2e x2e)
+          | Wf_rExpr {t} G (e1 e2 : expr t)
+            : expr.wf G e1 e2 -> wf_rawexpr G (rExpr e1) e1 (rExpr e2) e2
+          | Wf_rValue {t} G (v1 v2 : value t)
+            : wf_value G v1 v2
+              -> wf_rawexpr G (rValue v1) (reify v1) (rValue v2) (reify v2).
+
+          Lemma wf_rawexpr_Proper_list G1 G2
+                (HG1G2 : forall t v1 v2, List.In (existT _ t (v1, v2)) G1 -> List.In (existT _ t (v1, v2)) G2)
+                t re1 e1 re2 e2
+                (Hwf : @wf_rawexpr G1 t re1 e1 re2 e2)
+            : @wf_rawexpr G2 t re1 e1 re2 e2.
+          Proof.
+            revert dependent G2; induction Hwf; intros; constructor; eauto.
+            { eapply expr.wf_Proper_list; eauto. }
+            { eapply wf_value'_Proper_list; eauto. }
+          Qed.
+
+          (* Because [proj1] and [proj2] in the stdlib are opaque *)
+          Local Notation proj1 x := (let (a, b) := x in a).
+          Local Notation proj2 x := (let (a, b) := x in b).
+
+          Definition eq_type_of_rawexpr_of_wf {t G re1 e1 re2 e2} (Hwf : @wf_rawexpr G t re1 e1 re2 e2)
+            : type_of_rawexpr re1 = t /\ type_of_rawexpr re2 = t.
+          Proof. split; destruct Hwf; reflexivity. Defined.
+
+          Definition eq_expr_of_rawexpr_of_wf {t G re1 e1 re2 e2} (Hwf : @wf_rawexpr G t re1 e1 re2 e2)
+            : (rew [expr] (proj1 (eq_type_of_rawexpr_of_wf Hwf)) in expr_of_rawexpr re1) = e1
+              /\ (rew [expr] (proj2 (eq_type_of_rawexpr_of_wf Hwf)) in expr_of_rawexpr re2) = e2.
+          Proof. split; destruct Hwf; reflexivity. Defined.
+
+          Definition eq_expr_of_rawexpr_of_wf' {t G re1 e1 re2 e2} (Hwf : @wf_rawexpr G t re1 e1 re2 e2)
+            : expr_of_rawexpr re1 = (rew [expr] (eq_sym (proj1 (eq_type_of_rawexpr_of_wf Hwf))) in e1)
+              /\ expr_of_rawexpr re2 = (rew [expr] (eq_sym (proj2 (eq_type_of_rawexpr_of_wf Hwf))) in e2).
+          Proof. split; destruct Hwf; reflexivity. Defined.
+
+          Lemma wf_expr_of_wf_rawexpr {t G re1 e1 re2 e2} (Hwf : @wf_rawexpr G t re1 e1 re2 e2)
+            : expr.wf G e1 e2.
+          Proof. induction Hwf; repeat (assumption || constructor || apply wf_reify). Qed.
+
+          Lemma wf_expr_of_wf_rawexpr' {t G re1 e1 re2 e2} (Hwf : @wf_rawexpr G t re1 e1 re2 e2)
+            : expr.wf G
+                      (rew [expr] (proj1 (eq_type_of_rawexpr_of_wf Hwf)) in expr_of_rawexpr re1)
+                      (rew [expr] (proj2 (eq_type_of_rawexpr_of_wf Hwf)) in expr_of_rawexpr re2).
+          Proof.
+            pose proof Hwf as Hwf'.
+            rewrite <- (proj1 (eq_expr_of_rawexpr_of_wf Hwf)) in Hwf'.
+            rewrite <- (proj2 (eq_expr_of_rawexpr_of_wf Hwf)) in Hwf'.
+            eapply wf_expr_of_wf_rawexpr; eassumption.
+          Qed.
+
+          Lemma wf_value_of_wf_rawexpr {t G re1 e1 re2 e2} (Hwf : @wf_rawexpr G t re1 e1 re2 e2)
+            : wf_value G
+                       (rew [value] (proj1 (eq_type_of_rawexpr_of_wf Hwf)) in value_of_rawexpr re1)
+                       (rew [value] (proj2 (eq_type_of_rawexpr_of_wf Hwf)) in value_of_rawexpr re2).
+          Proof.
+            pose proof (wf_expr_of_wf_rawexpr Hwf).
+            destruct Hwf; cbn; try eapply wf_reflect; try assumption.
+          Qed.
+
+          Lemma reveal_rawexpr_cps_id {var} e T k
+            : @reveal_rawexpr_cps ident var e T k = k (reveal_rawexpr e).
+          Proof.
+            cbv [reveal_rawexpr_cps]; break_innermost_match; try reflexivity.
+            cbv [value value'] in *; expr.invert_match; try reflexivity.
+          Qed.
+
+          Lemma wf_reveal_rawexpr t G re1 e1 re2 e2 (Hwf : @wf_rawexpr G t re1 e1 re2 e2)
+            : @wf_rawexpr G t (reveal_rawexpr re1) e1 (reveal_rawexpr re2) e2.
+          Proof.
+            pose proof (wf_expr_of_wf_rawexpr Hwf).
+            destruct Hwf; cbv [reveal_rawexpr_cps id];
+              repeat first [ assumption
+                           | constructor
+                           | progress subst
+                           | progress cbn [reify eq_rect value value'] in *
+                           | progress destruct_head'_sig
+                           | progress destruct_head'_and
+                           | break_innermost_match_step
+                           | progress expr.invert_match
+                           | progress expr.inversion_wf_constr ].
+
+          Qed.
+
+          Fixpoint wf_pbase_type_interp_cps (quant : quant_type) (t1 t2 : pattern.base.type) (K1 K2 : base.type -> Type)
+                   (P : forall t, K1 t -> K2 t -> Prop) {struct t1}
+            : pbase_type_interp_cps quant t1 K1 -> pbase_type_interp_cps quant t2 K2 -> Prop
+            := match t1, t2, quant with
+               | pattern.base.type.any, pattern.base.type.any, qforall
+                 => fun v1 v2
+                    => forall t : base.type, P _ (v1 t) (v2 t)
+               | pattern.base.type.any, pattern.base.type.any, qexists
+                 => fun v1 v2
+                    => { pf : projT1 v1 = projT1 v2 | P _ (rew pf in projT2 v1) (projT2 v2) }
+               | pattern.base.type.type_base t1, pattern.base.type.type_base t2, _
+                 => fun v1 v2
+                    => { pf : t1 = t2 | P _ (rew [fun t : base.type.base => K1 t] pf in v1) v2 }
+               | pattern.base.type.prod A1 B1, pattern.base.type.prod A2 B2, _
+                 => @wf_pbase_type_interp_cps
+                      quant A1 A2 _ _
+                      (fun A' => @wf_pbase_type_interp_cps
+                                   quant B1 B2 _ _
+                                   (fun B' => P (A' * B')%etype))
+               | pattern.base.type.list A1, pattern.base.type.list A2, _
+                 => @wf_pbase_type_interp_cps
+                      quant A1 A2 _ _
+                      (fun A' => P (base.type.list A'))
+               | pattern.base.type.any, _, _
+               | pattern.base.type.type_base _, _, _
+               | pattern.base.type.prod _ _, _, _
+               | pattern.base.type.list _, _, _
+                 => fun _ _ => False
+               end.
+
+          Fixpoint wf_ptype_interp_cps (quant : quant_type) (t1 t2 : pattern.type) (K1 K2 : type -> Type)
+                   (P : forall t, K1 t -> K2 t -> Prop) {struct t1}
+            : ptype_interp_cps quant t1 K1 -> ptype_interp_cps quant t2 K2 -> Prop
+            := match t1, t2 with
+               | type.base t1, type.base t2 => wf_pbase_type_interp_cps quant t1 t2 _ _ (fun t => P (type.base t))
+               | type.arrow s1 d1, type.arrow s2 d2
+                 => wf_ptype_interp_cps
+                      quant s1 s2 _ _
+                      (fun s => wf_ptype_interp_cps
+                                  quant d1 d2 _ _
+                                  (fun d => P (type.arrow s d)))
+               | type.base _, _
+               | type.arrow _ _, _
+                 => fun _ _ => False
+               end.
+
+          Definition wf_ptype_interp_id G {quant t1 t2} : @ptype_interp var1 quant t1 id -> @ptype_interp var2 quant t2 id -> Prop
+            := @wf_ptype_interp_cps quant t1 t2 _ _ (@wf_value G).
+
+          Fixpoint wf_binding_dataT G (p1 p2 : pattern) : @binding_dataT var1 p1 -> @binding_dataT var2 p2 -> Prop
+            := match p1, p2 with
+               | pattern.Wildcard t1, pattern.Wildcard t2
+                 => wf_ptype_interp_id G
+               | pattern.Ident idc1, pattern.Ident idc2
+                 => fun v1 v2
+                    => { pf : idc1 = idc2 | (rew [fun idc => @binding_dataT _ (pattern.Ident idc)] pf in v1) = v2 }
+               | pattern.App f1 x1, pattern.App f2 x2
+                 => fun v1 v2
+                    => @wf_binding_dataT G _ _ (fst v1) (fst v2) /\ @wf_binding_dataT G _ _ (snd v1) (snd v2)
+               | pattern.Wildcard _, _
+               | pattern.Ident _, _
+               | pattern.App _ _, _
+                 => fun _ _ => False
+               end.
+
+          Lemma bind_base_cps_id t1 t2 K v T k
+            : @bind_base_cps t1 t2 K v T k = k (@bind_base_cps t1 t2 K v _ id).
+          Proof using Type.
+            revert t2 K v T k; induction t1, t2; intros; cbn [bind_base_cps]; try reflexivity;
+              rewrite_type_transport_correct; break_innermost_match; try reflexivity;
+                repeat first [ progress subst
+                             | progress inversion_option
+                             | reflexivity
+                             | match goal with
+                               | [ H : _ |- _ ] => rewrite H; (reflexivity || break_innermost_match_step)
+                               end ].
+          Qed.
+
+          Lemma wf_bind_base t1 t1' t2 t2' K1 K2 v1 v2 (Ht1 : t1 = t2) (Ht2 : t1' = t2') (P : forall t, K1 t -> K2 t -> Prop)
+                (Pv : P _ (rew Ht2 in v1) v2)
+            : option_eq (@wf_pbase_type_interp_cps _ _ _ _ _ P) (@bind_base_cps t1 t1' K1 v1 _ id) (@bind_base_cps t2 t2' K2 v2 _ id).
+          Proof.
+            subst t2' t2; revert t1' K1 v1 K2 v2 P Pv.
+            induction t1, t1'; cbn [wf_pbase_type_interp_cps bind_base_cps]; intros; cbv [cpsreturn id cpsbind cpscall cps_option_bind];
+              cbn [option_eq projT1 projT2];
+              repeat first [ (exists eq_refl)
+                           | reflexivity
+                           | progress subst
+                           | progress base.type.inversion_type
+                           | progress destruct_head' False
+                           | congruence
+                           | progress cbn [eq_rect option_eq] in *
+                           | progress cbv [id] in *
+                           | solve [ eauto ]
+                           | progress rewrite_type_transport_correct
+                           | progress type_beq_to_eq
+                           | progress break_match_step ltac:(fun v => let h := head v in constr_eq h (@Sumbool.sumbool_of_bool))
+                           | rewrite bind_base_cps_id; set (@bind_base_cps _ _ _ _ _ id) at 1
+                           | match goal with
+                             | [ H : forall P : (forall x, _ -> _ -> Prop), P _ _ _ -> False |- _ ]
+                               => specialize (H (fun _ _ _ => True) I)
+                             | [ H : forall P : (forall x, _ -> _ -> Prop), P _ _ _ -> Some _ = None |- _ ]
+                               => specialize (H (fun _ _ _ => True) I)
+                             | [ X := Some _ |- _ ] => subst X
+                             | [ X := None |- _ ] => subst X
+                             | [ HP : context[?P _ ?v1 ?v2], H' : _, X := @bind_base_cps ?t1 ?t2 ?K1 ?v1 _ (fun x => x), Y := @bind_base_cps ?t1' ?t2 ?K2 ?v2 _ (fun y => y) |- _ ]
+                               => specialize (H' t2 K1 v1 K2 v2);
+                                  destruct (@bind_base_cps t1 t2 K1 v1 _ (fun x => x)) eqn:?,
+                                           (@bind_base_cps t1' t2 K2 v2 _ (fun x => x)) eqn:?
+                             end ].
+          Qed.
+
+          Lemma bind_value_cps_id t1 t2 K v T k
+            : @bind_value_cps t1 t2 K v T k = k (@bind_value_cps t1 t2 K v _ id).
+          Proof using Type.
+            revert t2 K v T k; induction t1, t2; intros; cbn [bind_value_cps]; try reflexivity; [ apply bind_base_cps_id | ].
+            cbv [cps_option_bind cpscall cpsreturn cpsbind].
+            repeat first [ progress subst
+                         | progress inversion_option
+                         | reflexivity
+                         | match goal with
+                           | [ H : _ |- _ ] => rewrite H; (reflexivity || break_innermost_match_step)
+                           end ].
+          Qed.
+
+          Lemma wf_bind_value t1 t1' t2 t2' K1 K2 v1 v2 (Ht1 : t1 = t2) (Ht2 : t1' = t2') (P : forall t, K1 t -> K2 t -> Prop)
+                (Hv : P _ (rew Ht2 in v1) v2)
+            : option_eq (@wf_ptype_interp_cps _ _ _ _ _ P) (@bind_value_cps t1 t1' K1 v1 _ id) (@bind_value_cps t2 t2' K2 v2 _ id).
+          Proof.
+            subst t2' t2; revert t1' K1 v1 K2 v2 P Hv.
+            induction t1, t1'; cbn [wf_ptype_interp_cps bind_value_cps]; cbv [id cpsbind cpscall cpsreturn cps_option_bind];
+              cbn [option_eq]; intros; try reflexivity.
+            { unshelve eapply wf_bind_base; eauto. }
+            { repeat first [ progress destruct_head' False
+                           | congruence
+                           | progress cbn [eq_rect option_eq] in *
+                           | progress cbv [id] in *
+                           | solve [ eauto ]
+                           | rewrite bind_value_cps_id; set (@bind_value_cps _ _ _ _ _ id) at 1
+                           | match goal with
+                             | [ H : forall P : (forall x, _ -> _ -> Prop), P _ _ _ -> False |- _ ]
+                               => specialize (H (fun _ _ _ => True) I)
+                             | [ H : forall P : (forall x, _ -> _ -> Prop), P _ _ _ -> Some _ = None |- _ ]
+                               => specialize (H (fun _ _ _ => True) I)
+                             | [ X := Some _ |- _ ] => subst X
+                             | [ X := None |- _ ] => subst X
+                             | [ HP : context[?P _ ?v1 ?v2], H' : _, X := @bind_value_cps ?t1 ?t2 ?K1 ?v1 _ (fun x => x), Y := @bind_value_cps ?t1' ?t2 ?K2 ?v2 _ (fun y => y) |- _ ]
+                               => specialize (H' t2 K1 v1 K2 v2);
+                                  destruct (@bind_value_cps t1 t2 K1 v1 _ (fun x => x)) eqn:?,
+                                           (@bind_value_cps t1' t2 K2 v2 _ (fun x => x)) eqn:?
+                             end ]. }
+          Qed.
+
+          Lemma bind_data_cps_id {var} e p T k
+            : @bind_data_cps var e p T k = k (bind_data e p).
+          Proof using try_make_transport_ident_cps_correct.
+            revert p T k; induction e, p; intros; cbn [bind_data_cps]; try (reflexivity || apply bind_value_cps_id);
+              cbv [cps_option_bind cpscall cpsreturn cpsbind];
+              repeat first [ progress subst
+                           | progress inversion_option
+                           | reflexivity
+                           | rewrite try_make_transport_ident_cps_correct
+                           | match goal with
+                             | [ H : _ |- _ ] => rewrite H; (reflexivity || break_innermost_match_step)
+                             end
+                           | break_innermost_match_step ].
+          Qed.
+
+          Lemma wf_bind_data t G re1 e1 re2 e2 p1 p2 (Hwf : @wf_rawexpr G t re1 e1 re2 e2) (Hp : p1 = p2)
+            : option_eq (@wf_binding_dataT G p1 p2) (bind_data re1 p1) (bind_data re2 p2).
+          Proof.
+            subst p2; revert p1; induction Hwf, p1; cbn [bind_data_cps value_of_rawexpr];
+              rewrite_type_transport_correct;
+              rewrite ?try_make_transport_ident_cps_correct.
+            all: repeat first [ (exists eq_refl)
+                              | exact I
+                              | reflexivity
+                              | unshelve eapply wf_bind_value
+                              | progress break_match_step ltac:(fun v => let h := head v in constr_eq h (@Sumbool.sumbool_of_bool))
+                              | progress cbn [eq_rect wf_binding_dataT fst snd option_eq] in *
+                              | progress cbv [id] in *
+                              | progress subst
+                              | progress inversion_option
+                              | apply wf_reflect
+                              | match goal with
+                                | [ |- context[pident_bl ?a ?b ?pf] ] => generalize (pident_bl a b pf); intros
+                                | [ X := Some _ |- _ ] => subst X
+                                | [ X := None |- _ ] => subst X
+                                | [ X := @bind_data_cps _ ?e ?p _ (fun y => y), H : context[@bind_data_cps _ ?e _ _ (fun x => x)] |- _ ]
+                                  => pose proof (H p); destruct (@bind_data_cps _ e p _ (fun y => y)) eqn:?
+                                end
+                              | rewrite bind_data_cps_id; set (@bind_data _ _) at 1
+                              | solve [ auto ]
+                              | eapply wf_expr_of_wf_rawexpr; eassumption
+                              | wf_safe_t_step ].
+          Qed.
+
+          Lemma swap_list_None_iff {A} (i j : nat) (ls : list A)
+            : swap_list i j ls = None <-> (length ls <= i \/ length ls <= j)%nat.
+          Proof.
+            rewrite <- !nth_error_None.
+            cbv [swap_list]; break_innermost_match; intuition congruence.
+          Qed.
+
+          Lemma swap_list_Some_length {A} (i j : nat) (ls ls' : list A)
+            : swap_list i j ls = Some ls'
+              -> (i < length ls /\ j < length ls /\ length ls' = length ls)%nat.
+          Proof.
+            cbv [swap_list]; break_innermost_match; intros; inversion_option; subst.
+            repeat match goal with H : _ |- _ => apply nth_error_value_length in H end.
+            autorewrite with distr_length; tauto.
+          Qed.
+
+          Local Ltac fin_handle_list :=
+            destruct_head' iff;
+            destruct_head'_and;
+            cbn [length] in *;
+            try solve [ destruct_head'_or;
+                        exfalso;
+                        repeat match goal with
+                               | [ H : ?T, H' : ?T |- _ ] => clear H'
+                               | [ H : ?T |- _ ]
+                                 => lazymatch type of H with
+                                    | _ = _ :> nat => fail
+                                    | (_ <= _)%nat => fail
+                                    | (_ < _)%nat => fail
+                                    | ~_ = _ :> nat => fail
+                                    | ~(_ <= _)%nat => fail
+                                    | ~(_ < _)%nat => fail
+                                    | _ => clear H
+                                    end
+                               | [ H : context[length ?ls] |- _ ]
+                                 => generalize dependent (length ls); intros
+                               | _ => progress subst
+                               | _ => lia
+                               end ].
+
+          Local Ltac handle_nth_error :=
+            repeat match goal with
+                   | [ H : nth_error _ _ = None |- _ ] => rewrite nth_error_None in H
+                   | [ H : nth_error _ _ = Some _ |- _ ] => unique pose proof (@nth_error_value_length _ _ _ _ H)
+                   end;
+            fin_handle_list.
+
+          Lemma nth_error_swap_list {A} {i j : nat} {ls ls' : list A}
+            : swap_list i j ls = Some ls'
+              -> forall k,
+                nth_error ls' k = if Nat.eq_dec k i then nth_error ls j else if Nat.eq_dec k j then nth_error ls i else nth_error ls k.
+          Proof.
+            cbv [swap_list]; break_innermost_match; intros; inversion_option; subst;
+              rewrite ?nth_set_nth; distr_length; break_innermost_match; try congruence; try lia;
+                handle_nth_error.
+          Qed.
+
+          Local Ltac handle_swap_list :=
+            repeat match goal with
+                   | [ H : swap_list _ _ _ = None |- _ ] => rewrite swap_list_None_iff in H
+                   | [ H : swap_list _ _ _ = Some _ |- _ ] => unique pose proof (@swap_list_Some_length _ _ _ _ _ H)
+                   end;
+            fin_handle_list.
+
+          Fixpoint wf_eval_decision_tree' {T1 T2} G d (P : option T1 -> option T2 -> Prop) (HPNone : P None None) {struct d}
+            : forall (ctx1 : list (@rawexpr var1))
+                     (ctx2 : list (@rawexpr var2))
+                     (ctxe : list { t : type & @expr var1 t * @expr var2 t }%type)
+                     (Hctx1 : length ctx1 = length ctxe)
+                     (Hctx2 : length ctx2 = length ctxe)
+                     (Hwf : forall t re1 e1 re2 e2,
+                         List.In ((re1, re2), existT _ t (e1, e2)) (List.combine (List.combine ctx1 ctx2) ctxe)
+                         -> @wf_rawexpr G t re1 e1 re2 e2)
+                     cont1 cont2
+                     (Hcont : forall n ls1 ls2,
+                         length ls1 = length ctxe
+                         -> length ls2 = length ctxe
+                         -> (forall t re1 e1 re2 e2,
+                                List.In ((re1, re2), existT _ t (e1, e2)) (List.combine (List.combine ls1 ls2) ctxe)
+                                -> @wf_rawexpr G t re1 e1 re2 e2)
+                         -> (cont1 n ls1 = None <-> cont2 n ls2 = None)
+                            /\ P (cont1 n ls1) (cont2 n ls2)),
+              ((@eval_decision_tree var1 T1 ctx1 d cont1) = None <-> (@eval_decision_tree var2 T2 ctx2 d cont2) = None)
+              /\ P (@eval_decision_tree var1 T1 ctx1 d cont1) (@eval_decision_tree var2 T2 ctx2 d cont2).
+          Proof using pident_to_typed_invert_bind_args.
+            clear -HPNone pident_to_typed_invert_bind_args wf_eval_decision_tree'.
+            specialize (fun d => wf_eval_decision_tree' T1 T2 G d P HPNone).
+            destruct d; cbn [eval_decision_tree]; intros; try (clear wf_eval_decision_tree'; tauto).
+            { let d := match goal with d : decision_tree |- _ => d end in
+              specialize (wf_eval_decision_tree' d).
+              cbv [Option.sequence Option.bind Option.sequence_return];
+                break_innermost_match;
+                specialize_all_ways;
+                handle_swap_list;
+                repeat first [ assumption
+                             | match goal with
+                               | [ H : ?T, H' : ?T |- _ ] => clear H'
+                               end
+                             | progress inversion_option
+                             | progress destruct_head'_and
+                             | progress destruct_head' iff
+                             | progress specialize_by_assumption
+                             | progress cbn [length] in *
+                             | match goal with
+                               | [ H : ?x = Some _, H' : context[?x] |- _ ] => rewrite H in H'
+                               | [ H : ?x = None, H' : context[?x] |- _ ] => rewrite H in H'
+                               | [ H : length ?x = length ?y, H' : context[length ?x] |- _ ] => rewrite H in H'
+                               | [ H : S _ = S _ |- _ ] => inversion H; clear H
+                               | [ H : S _ = length ?ls |- _ ] => is_var ls; destruct ls; cbn [length] in H; inversion H; clear H
+                               end
+                             | congruence
+                             | apply conj
+                             | progress intros
+                             | progress destruct_head'_or ]. }
+            { let d := match goal with d : decision_tree |- _ => d end in
+              pose proof (wf_eval_decision_tree' d) as IHd.
+              let d := match goal with d : option decision_tree |- _ => d end in
+              pose proof (match d as d' return match d' with Some _ => _ | None => True end with
+                          | Some d => wf_eval_decision_tree' d
+                          | None => I
+                          end) as IHapp_case.
+              all: destruct ctx1, ctx2; cbn [length] in *; try (clear wf_eval_decision_tree'; (tauto || congruence)); [].
+              all: lazymatch goal with
+                   | [ |- _
+                          /\ ?P match ?d with
+                                | TryLeaf _ _ => (?res1 ;; ?ev1)%option
+                                | _ => _
+                                end
+                              match ?d with
+                              | TryLeaf _ _ => (?res2 ;; ?ev2)%option
+                              | _ => _
+                              end ]
+                     => cut (((res1 = None <-> res2 = None) /\ P res1 res2) /\ ((ev1 = None <-> ev2 = None) /\ P ev1 ev2));
+                          [ clear wf_eval_decision_tree';
+                            intro; destruct_head'_and; destruct_head' iff;
+                            destruct d; destruct res1 eqn:?, res2 eqn:?; cbn [Option.sequence];
+                            solve [ intuition (congruence || eauto) ] | ]
+                   end.
+              all: split; [ | clear wf_eval_decision_tree'; eapply IHd; eassumption ].
+              (** We use the trick that [induction] inside [Fixpoint]
+                  gives us nested [fix]es that pass the guarded
+                  checker, as long as we're careful about how we do
+                  things *)
+              let icases := match goal with d : list (_ * decision_tree) |- _ => d end in
+              induction icases as [|icase icases IHicases];
+                [ | pose proof (wf_eval_decision_tree' (snd icase)) as IHicase ];
+                clear wf_eval_decision_tree'.
+              (** now we can stop being super-careful about [destruct]
+                  ordering because, if we're [Guarded] here (which we
+                  are), then we cannot break guardedness from this
+                  point on, because we've cleared the bare fixpoint
+                  after specializing it to valid arguments *)
+              2: revert IHicases.
+              all: repeat (rewrite reveal_rawexpr_cps_id; set (reveal_rawexpr _)).
+              all: repeat match goal with H := reveal_rawexpr _ |- _ => subst H end.
+              all: repeat first [ match goal with
+                                  | [ H : S _ = S _ |- _ ] => inversion H; clear H
+                                  | [ H : S _ = length ?ls |- _ ] => is_var ls; destruct ls; cbn [length] in H; inversion H; clear H
+                                  | [ H : forall t re1 e1 re2 e2, _ = _ \/ _ -> _ |- _ ]
+                                    => pose proof (H _ _ _ _ _ (or_introl eq_refl));
+                                       specialize (fun t re1 e1 re2 e2 pf => H t re1 e1 re2 e2 (or_intror pf))
+                                  | [ H : wf_rawexpr ?G ?r ?e ?r' ?e' |- context[reveal_rawexpr ?r] ]
+                                    => apply wf_reveal_rawexpr in H; revert H;
+                                       generalize (reveal_rawexpr r) (reveal_rawexpr r'); clear r r'; intros r r' H; destruct H
+                                  | [ H1 : length ?ctx1 = length ?ctxe', H2 : length ?ctx2 = length ?ctxe', H1' : wf_rawexpr _ ?f1 ?f1e ?f2 ?f2e, H2' : wf_rawexpr _ ?x1 ?x1e ?x2 ?x2e
+                                      |- _ /\ ?P (@eval_decision_tree _ _ (?f1 :: ?x1 :: ?ctx1) _ _)
+                                               (@eval_decision_tree _ _ (?f2 :: ?x2 :: ?ctx2) _ _) ]
+                                    => apply IHapp_case with (ctxe:=existT _ _ (f1e, f2e) :: existT _ _ (x1e, x2e) :: ctxe'); clear IHapp_case
+                                  | [ H : ?x = ?x -> _ |- _ ] => specialize (H eq_refl)
+                                  | [ H : ?x = ?x |- _ ] => clear H
+                                  | [ |- context [pident_to_typed_invert_bind_args_type ?t ?idc ?p ?f ?pf] ]
+                                    => generalize (type_of_pident p f) (pident_to_typed_invert_bind_args_type t idc p f pf); clear p f pf; intros; subst
+                                  end
+                                | tauto
+                                | progress subst
+                                | progress cbn [length combine List.In fold_right fst snd projT1 projT2 eq_rect Option.sequence Option.sequence_return eq_rect] in *
+                                | progress inversion_sigma
+                                | progress inversion_prod
+                                | progress destruct_head'_sigT
+                                | progress destruct_head'_prod
+                                | progress destruct_head'_and
+                                | progress destruct_head' iff; progress specialize_by (exact eq_refl)
+                                | congruence
+                                | break_innermost_match_step
+                                | progress intros
+                                | progress destruct_head'_or
+                                | solve [ auto ]
+                                | match goal with
+                                  | [ |- wf_rawexpr _ _ _ _ _ ] => constructor
+                                  | [ H : context[(_ = None <-> _ = None) /\ ?P _ _] |- (_ = None <-> _ = None) /\ ?P _ _ ]
+                                    => apply H
+                                  | [ H : fold_right _ None ?ls = None, H' : fold_right _ None ?ls = Some None |- _ ]
+                                    => exfalso; clear -H H'; is_var ls; destruct ls; cbn [fold_right] in H, H'; break_match_hyps; congruence
+                                  end
+                                | progress break_match
+                                | progress cbv [option_bind' Option.bind]
+                                | unshelve erewrite pident_to_typed_invert_bind_args; [ shelve | shelve | eassumption | ]
+                                | match goal with
+                                  | [ |- _ /\ ?P (Option.sequence ?x ?y) (Option.sequence ?x' ?y') ]
+                                    => cut ((x = None <-> x' = None) /\ P x x');
+                                       [ destruct x, x'; cbn [Option.sequence]; solve [ intuition congruence ] | ]
+                                  | [ H1 : length ?ctx1 = length ?ctxe', H2 : length ?ctx2 = length ?ctxe'
+                                      |- _ /\ ?P (@eval_decision_tree _ _ ?ctx1 _ _) (@eval_decision_tree _ _ ?ctx2 _ _) ]
+                                    => apply IHicase with (ctxe := ctxe'); auto
+                                  end ]. }
+            { let d := match goal with d : decision_tree |- _ => d end in
+              specialize (wf_eval_decision_tree' d); rename wf_eval_decision_tree' into IHd.
+              break_innermost_match; handle_swap_list; try tauto; [].
+              lazymatch goal with
+              | [ H : swap_list ?i ?j _ = _ |- _ ] => destruct (swap_list i j ctxe) as [ctxe'|] eqn:?
+              end; handle_swap_list; [].
+              eapply IHd with (ctxe:=ctxe'); clear IHd; try congruence;
+                [ | intros; break_innermost_match; handle_swap_list; apply Hcont; try congruence; [] ]; clear Hcont.
+              all: intros ? ? ? ? ? HIn.
+              1: eapply Hwf; clear Hwf.
+              2: lazymatch goal with
+                 | [ H : context[List.In _ (combine _ ctxe') -> wf_rawexpr _ _ _ _ _] |- _ ] => apply H; clear H
+                 end.
+              all: apply In_nth_error_value in HIn; destruct HIn as [n' HIn].
+              all: lazymatch goal with
+                   | [ H : swap_list ?i ?j _ = _ |- _ ]
+                     => apply nth_error_In with (n:=if Nat.eq_dec i n' then j else if Nat.eq_dec j n' then i else n')
+                   end.
+              all: repeat first [ reflexivity
+                                | match goal with
+                                  | [ H : context[nth_error (combine _ _) _] |- _ ] => rewrite !nth_error_combine in H
+                                  | [ |- context[nth_error (combine _ _) _] ] => rewrite !nth_error_combine
+                                  | [ H : swap_list _ _ ?ls = Some ?ls', H' : context[nth_error ?ls' ?k] |- _ ]
+                                    => rewrite (nth_error_swap_list H) in H'
+                                  | [ H : nth_error ?ls ?k = _, H' : context[nth_error ?ls ?k] |- _ ] => rewrite H in H'
+                                  end
+                                | progress subst
+                                | progress inversion_option
+                                | progress inversion_prod
+                                | congruence
+                                | progress handle_nth_error
+                                | break_innermost_match_step
+                                | break_innermost_match_hyps_step ]. }
+          Qed.
+
+          Lemma wf_eval_decision_tree {T1 T2} G d (P : option T1 -> option T2 -> Prop) (HPNone : P None None)
+            : forall (ctx1 : list (@rawexpr var1))
+                     (ctx2 : list (@rawexpr var2))
+                     (ctxe : list { t : type & @expr var1 t * @expr var2 t }%type)
+                     (Hctx1 : length ctx1 = length ctxe)
+                     (Hctx2 : length ctx2 = length ctxe)
+                     (Hwf : forall t re1 e1 re2 e2,
+                         List.In ((re1, re2), existT _ t (e1, e2)) (List.combine (List.combine ctx1 ctx2) ctxe)
+                         -> @wf_rawexpr G t re1 e1 re2 e2)
+                     cont1 cont2
+                     (Hcont : forall n ls1 ls2,
+                         length ls1 = length ctxe
+                         -> length ls2 = length ctxe
+                         -> (forall t re1 e1 re2 e2,
+                                List.In ((re1, re2), existT _ t (e1, e2)) (List.combine (List.combine ls1 ls2) ctxe)
+                                -> @wf_rawexpr G t re1 e1 re2 e2)
+                         -> (cont1 n ls1 = None <-> cont2 n ls2 = None)
+                            /\ P (cont1 n ls1) (cont2 n ls2)),
+              P (@eval_decision_tree var1 T1 ctx1 d cont1) (@eval_decision_tree var2 T2 ctx2 d cont2).
+          Proof using pident_to_typed_invert_bind_args. intros; eapply wf_eval_decision_tree'; eassumption. Qed.
+
+
+          (*
+        Local Notation opt_anyexprP ivar
+          := (fun should_do_again : bool => UnderLets (@AnyExpr.anyexpr base.type ident (if should_do_again then ivar else var)))
+               (only parsing).
+        Local Notation opt_anyexpr ivar
+          := (option (sigT (opt_anyexprP ivar))) (only parsing).
+
+        Definition rewrite_ruleTP
+          := (fun p : pattern => binding_dataT p -> forall T, (opt_anyexpr value -> T) -> T).
+        Definition rewrite_ruleT := sigT rewrite_ruleTP.
+        Definition rewrite_rulesT
+          := (list rewrite_ruleT).
+
+        Definition ERROR_BAD_REWRITE_RULE {t} (pat : pattern) (value : expr t) : expr t. exact value. Qed.
+           *)
+
+          (*
+          Fixpoint natural_type_of_pattern_binding_data {var} (p : pattern) : @binding_dataT var p -> option { t : type & @expr var t }.
+          Proof.
+            refine match p with
+                   | pattern.Wildcard t => _
+                   | pattern.Ident idc => _
+                   | pattern.App f x => _
+                   end.
+            all: cbn.
+            Focus 2.
+            Fixpoint natural_of_ptype_interp {var} (t : ptype) k (K : forall t, k t -> option { t : type & @expr var t }) {struct t}
+              : @ptype_interp var qexists t k -> option { t : type & @expr var t }.
+              refine match t with
+                     | type.base t => _
+                     | type.arrow s d => _
+                     end.
+              all: cbn.
+              Focus 2.
+              Fixpoint natural_of_pbase_type_interp {var} (t : ptype) k (K : forall t, k t -> option { t : type & @expr var t }) {struct t}
+              : @ptype_interp var qexists t k -> option { t : type & @expr var t }.
+              refine match t with
+                     | type.base t => _
+                     | type.arrow s d => _
+                     end.
+              all: cbn.
+              refine
+          Proof.
+            refine match p with
+                   | pattern.Wildcard t => _
+                   | pattern.Ident idc => _
+                   | pattern.App f x => _
+                   end.
+            cbn.
+
+           *)
+
+          Definition rewrite_rules_goodT
+                     (rew1 : rewrite_rulesT1) (rew2 : rewrite_rulesT2)
+            : Prop
+            := length rew1 = length rew2
+               /\ (forall p r, List.In (existT _ p r) rew1 -> forall v T k, r v T k = k (r v _ id))
+               /\ (forall p r, List.In (existT _ p r) rew2 -> forall v T k, r v T k = k (r v _ id))
+               /\ (forall p1 r1 p2 r2,
+                      List.In (existT _ p1 r1, existT _ p2 r2) (combine rew1 rew2)
+                      -> p1 = p2
+                         /\ (forall G v1 v2,
+                                wf_binding_dataT G p1 p2 v1 v2
+                                -> option_eq
+                                     (fun rv1 rv2
+                                      => exists t : base.type, (* TODO: FIXME: This should be the natural type of the rewrite rule, probably *)
+                                          match projT1 rv1 as sda1, projT1 rv2 as sda2
+                                                return UnderLets _ (@AnyExpr.anyexpr base.type ident (if sda1 then _ else _))
+                                                       -> UnderLets _ (@AnyExpr.anyexpr base.type ident (if sda2 then _ else _))
+                                                       -> Prop
+                                          with
+                                          | true, true
+                                            => UnderLets.wf
+                                                 (fun G' v1 v2
+                                                  => exists (pf1 : anyexpr_ty v1 = t) (pf2 : anyexpr_ty v2 = t),
+                                                      forall G'',
+                                                        (forall t' v1' v2', List.In (existT _ t' (v1', v2')) G'' -> wf_value G v1' v2')
+                                                        -> expr.wf G''
+                                                                   (rew [fun t : base.type => expr t] pf1 in unwrap v1)
+                                                                   (rew [fun t : base.type => expr t] pf2 in unwrap v2))
+                                                 G
+                                          | false, false
+                                            => UnderLets.wf (fun G' => wf_anyexpr G' t) G
+                                          | true, false | false, true => fun _ _ => False
+                                          end (projT2 rv1) (projT2 rv2))
+                                     (r1 v1 _ id)
+                                     (r2 v2 _ id))).
+
+          Local Ltac do_eq_type_of_rawexpr_of_wf :=
+            repeat first [ match goal with
+                           | [ |- context[rew [fun t => UnderLets ?var (@?P t)] ?pf in UnderLets.Base ?v] ]
+                             => rewrite <- (fun x y p => @Equality.ap_transport _ P (fun t => UnderLets var (P t)) x y p (fun _ => UnderLets.Base))
+                           | [ |- UnderLets.wf _ _ _ _ ] => constructor
+                           | [ |- (?x = ?x <-> ?y = ?y) /\ _ ] => split; [ tauto | ]
+                           end
+                         | apply wf_expr_of_wf_rawexpr' ].
+          Local Ltac solve_eq_type_of_rawexpr_of_wf := solve [ do_eq_type_of_rawexpr_of_wf ].
+
+          Local Ltac gen_do_eq_type_of_rawexpr_of_wf :=
+            match goal with
+            | [ |- context[eq_type_of_rawexpr_of_wf ?Hwf] ]
+              => let H' := fresh in
+                 pose proof (wf_expr_of_wf_rawexpr Hwf) as H';
+                 rewrite <- (proj1 (eq_expr_of_rawexpr_of_wf Hwf)),  <- (proj2 (eq_expr_of_rawexpr_of_wf Hwf)) in H';
+                 destruct Hwf; cbn in H'; cbn [eq_type_of_rawexpr_of_wf eq_rect expr_of_rawexpr type_of_rawexpr]
+            end.
+
+          (* move me? *)
+          Local Lemma ap_transport_splice {var T}
+                (A B : T -> Type)
+                (x y : T) (p : x = y)
+                (v : @UnderLets var (A x)) (f : A x -> @UnderLets var (B x))
+            : (rew [fun t => @UnderLets var (B t)] p in UnderLets.splice v f)
+              = UnderLets.splice (rew [fun t => @UnderLets var (A t)] p in v)
+                                 (fun v => rew [fun t => @UnderLets var (B t)] p in f (rew [A] (eq_sym p) in v)).
+          Proof. case p; reflexivity. Defined.
+
+          Local Transparent ERROR_BAD_REWRITE_RULE.
+          Lemma ERROR_BAD_REWRITE_RULE_id {var t p v} : @ERROR_BAD_REWRITE_RULE ident var pident t p v = v.
+          Proof. exact eq_refl. Qed.
+          Local Opaque ERROR_BAD_REWRITE_RULE.
+
+          Lemma wf_eval_rewrite_rules
+                (do_again1 : forall t : base.type, @expr.expr base.type ident (@value var1) t -> @UnderLets var1 (@expr var1 t))
+                (do_again2 : forall t : base.type, @expr.expr base.type ident (@value var2) t -> @UnderLets var2 (@expr var2 t))
+                (wf_do_again : forall G (t : base.type) e1 e2,
+                    expr.wf nil e1 e2
+                    -> UnderLets.wf (fun G' => expr.wf G') G (@do_again1 t e1) (@do_again2 t e2))
+                (d : @decision_tree pident)
+                (rew1 : rewrite_rulesT1) (rew2 : rewrite_rulesT2)
+                (Hrew : rewrite_rules_goodT rew1 rew2)
+                (re1 : @rawexpr var1) (re2 : @rawexpr var2)
+                {t} G e1 e2
+                (Hwf : @wf_rawexpr G t re1 e1 re2 e2)
+            : UnderLets.wf
+                (fun G' => expr.wf G')
+                G
+                (rew [fun t => @UnderLets var1 (expr t)] (proj1 (eq_type_of_rawexpr_of_wf Hwf)) in (eval_rewrite_rules1 do_again1 d rew1 re1))
+                (rew [fun t => @UnderLets var2 (expr t)] (proj2 (eq_type_of_rawexpr_of_wf Hwf)) in (eval_rewrite_rules2 do_again2 d rew2 re2)).
+          Proof.
+            cbv [eval_rewrite_rules Option.sequence_return].
+            cbv [rewrite_rules_goodT] in Hrew.
+            eapply wf_eval_decision_tree with (ctxe:=[existT _ t (e1, e2)]);
+              cbn [length combine];
+              try solve [ reflexivity
+                        | cbn [combine In]; wf_t; tauto ].
+            all: repeat first [ progress do_eq_type_of_rawexpr_of_wf
+                              | match goal with
+                                | [ |- (Some _ = None <-> Some _ = None) /\ _ ] => split; [ clear; solve [ intuition congruence ] | ]
+                                | [ Hrew : length _ = length _, H : nth_error _ _ = None, H' : nth_error _ _ = Some _ |- _ ]
+                                  => exfalso; rewrite nth_error_None in H;
+                                     apply nth_error_value_length in H';
+                                     clear -Hrew H H'; try lia
+                                | [ |- context[rew [fun t => @UnderLets ?varp (@?P t)] ?pf in (@UnderLets.splice ?base_type ?ident ?var ?A ?B ?a ?b)] ]
+                                  => rewrite (@ap_transport_splice varp _ (fun _ => _) P _ _ pf a b
+                                              : (rew [fun t => @UnderLets varp (P t)] pf in (@UnderLets.splice base_type ident var A B a b)) = _)
+                                end
+                              | progress intros
+                              | progress subst
+                              | progress destruct_head'_and
+                              | progress destruct_head'_ex
+                              | progress destruct_head' False
+                              | progress split_and
+                              | progress specialize_by (exact eq_refl)
+                              | progress cbn [length combine In Option.bind option_eq fst snd projT1 projT2 UnderLets.splice anyexpr_ty unwrap eq_rect] in *
+                              | progress cbv [rewrite_ruleT id] in *
+                              | progress destruct_head'_sigT
+                              | rewrite Equality.transport_const
+                              | progress rewrite_type_transport_correct
+                              | progress type_beq_to_eq
+                              | congruence
+                              | progress destruct_head' (@wf_anyexpr)
+                              | progress destruct_head'_bool
+                              | progress break_match_step ltac:(fun v => let h := head v in constr_eq h (@Sumbool.sumbool_of_bool))
+                              | eapply UnderLets.wf_splice; [ solve [ eauto ] | ]
+                              | match goal with
+                                | [ H : S _ = S _ |- _ ] => inversion H; clear H
+                                | [ H : length ?ls = O |- _ ] => is_var ls; destruct ls
+                                | [ H : length ?ls = S _ |- _ ] => is_var ls; destruct ls
+                                | [ H : ?x = ?x |- _ ] => clear H
+                                | [ H : forall a b c d e, _ = _ \/ False -> _ |- _ ] => specialize (H _ _ _ _ _ (or_introl eq_refl))
+                                | [ |- context[@nth_error ?A ?ls ?n] ] => destruct (@nth_error A ls n) eqn:?
+                                | [ H : forall a b c d, In _ _ -> _, H' : nth_error _ ?n = Some _ |- _ ]
+                                  => specialize (fun a b c d pf => H a b c d (@nth_error_In _ _ n _ pf))
+                                | [ H : forall a b, In _ _ -> _, H' : nth_error _ ?n = Some _ |- _ ]
+                                  => specialize (fun a b pf => H a b (@nth_error_In _ _ n _ pf))
+                                | [ H : context[nth_error (combine ?l1 ?l2) ?n] |- _ ]
+                                  => rewrite (@nth_error_combine _ _ n) in H
+                                | [ H : ?x = Some _, H' : context[?x] |- _ ] => rewrite H in H'
+                                | [ H : forall a b c d, Some _ = Some _ -> _ |- _ ] => specialize (H _ _ _ _ eq_refl)
+                                | [ H : forall a b, Some _ = Some _ -> _ |- _ ] => specialize (H _ _ eq_refl)
+                                | [ H : forall v T k, ?f v T k = k (?f v _ (fun x => x)) |- context[?f ?v' ?T' ?k'] ]
+                                  => (tryif (let __ := constr:(eq_refl : k' = (fun x => x)) in idtac)
+                                       then fail
+                                       else rewrite (H v' T' k'))
+                                | [ H : forall G v1 v2, wf_binding_dataT G ?a ?b v1 v2 -> _, H' : wf_binding_dataT ?G' ?a ?b ?v1' ?v2' |- _ ]
+                                  => specialize (H _ _ _ H')
+                                | [ X := Some _ |- _ ] => subst X
+                                | [ X := None |- _ ] => subst X
+                                | [ X := @bind_data_cps ?var1 ?r1 ?p1 ?T1 (fun x => x), Y := @bind_data_cps ?var2 ?r2 ?p2 ?T2 (fun y => y) |- _ ]
+                                  => pose proof (fun Hp : p1 = p2 => @wf_bind_data _ _ r1 _ r2 _ p1 p2 ltac:(eassumption) Hp);
+                                     cbv [id] in *;
+                                     destruct (@bind_data_cps var1 r1 p1 T1 (fun x => x)), (@bind_data_cps var2 r2 p2 T2 (fun y => y))
+                                end
+                              | rewrite bind_data_cps_id; set (bind_data _ _)
+                              | match goal with
+                                | [ H : option_eq _ ?x ?y |- context[?x] ]
+                                  => destruct x eqn:?, y eqn:?; cbn [option_eq] in H
+                                | [ H : wf_value ?G ?v1 ?v2 |- wf_value' (?x0::?seg' ++ ?G) (?v1 _) (?v2 _) ]
+                                  => apply (H (x0::seg')); [ reflexivity | apply wf_reflect ]; solve [ wf_t ]
+                                | [ |- UnderLets.wf
+                                         _ _
+                                         (rew (proj1 (eq_type_of_rawexpr_of_wf ?Hwf)) in match type_of_rawexpr _ with _ => _ end _ _)
+                                         (rew (proj2 (eq_type_of_rawexpr_of_wf ?Hwf)) in match type_of_rawexpr _ with _ => _ end _ _) ]
+                                  => gen_do_eq_type_of_rawexpr_of_wf; break_innermost_match_step
+                                end
+                              | rewrite ERROR_BAD_REWRITE_RULE_id
+                              | wf_safe_t_step
+                              | eapply expr.wf_Proper_list; [ | eapply wf_expr_of_wf_rawexpr; eassumption ]; wf_t
+                              | eapply UnderLets.wf_splice; [ solve [ apply wf_do_again; wf_t ] | ]
+                              | apply wf_reify
+                              | progress destruct_head' (@AnyExpr.anyexpr)
+                              | rewrite app_assoc
+                              | progress fold (@reify var1) (@reify var2) (@reflect var1) (@reflect var2) ].
+          Qed.
+
+          (*
+        Fixpoint with_bindingsT (p : pattern) (T : Type)
+          := match p return Type with
+             | pattern.Wildcard t => ptype_interp qforall t (fun eT => eT -> T)
+             | pattern.Ident idc
+               => match arg_types idc with
+                 | Some t => t -> T
+                 | None => T
+                 end
+             | pattern.App f x => with_bindingsT f (with_bindingsT x T)
+             end.
+
+        Fixpoint lift_pbase_type_interp_cps {K1 K2} {quant} (F : forall t : base.type, K1 t -> K2 t) {t}
+          : pbase_type_interp_cps quant t K1
+            -> pbase_type_interp_cps quant t K2
+          := match t, quant return pbase_type_interp_cps quant t K1
+                                   -> pbase_type_interp_cps quant t K2 with
+             | pattern.base.type.any, qforall
+               => fun f t => F t (f t)
+             | pattern.base.type.any, qexists
+               => fun tf => existT _ _ (F _ (projT2 tf))
+             | pattern.base.type.type_base t, _
+               => F _
+             | pattern.base.type.prod A B, _
+               => @lift_pbase_type_interp_cps
+                   _ _ quant
+                   (fun A'
+                    => @lift_pbase_type_interp_cps
+                        _ _ quant (fun _ => F _) B)
+                   A
+             | pattern.base.type.list A, _
+               => @lift_pbase_type_interp_cps
+                   _ _ quant (fun _ => F _) A
+             end.
+
+        Fixpoint lift_ptype_interp_cps {K1 K2} {quant} (F : forall t : type.type base.type, K1 t -> K2 t) {t}
+          : ptype_interp_cps quant t K1
+            -> ptype_interp_cps quant t K2
+          := match t return ptype_interp_cps quant t K1
+                                   -> ptype_interp_cps quant t K2 with
+             | type.base t
+               => lift_pbase_type_interp_cps F
+             | type.arrow A B
+               => @lift_ptype_interp_cps
+                   _ _ quant
+                   (fun A'
+                    => @lift_ptype_interp_cps
+                        _ _ quant (fun _ => F _) B)
+                   A
+             end.
+
+        Fixpoint lift_with_bindings {p} {A B : Type} (F : A -> B) {struct p} : with_bindingsT p A -> with_bindingsT p B
+          := match p return with_bindingsT p A -> with_bindingsT p B with
+             | pattern.Wildcard t
+               => lift_ptype_interp_cps
+                   (K1:=fun t => value t -> A)
+                   (K2:=fun t => value t -> B)
+                   (fun _ f v => F (f v))
+             | pattern.Ident idc
+               => match arg_types idc as ty
+                       return match ty with
+                              | Some t => t -> A
+                              | None => A
+                              end -> match ty with
+                                    | Some t => t -> B
+                                    | None => B
+                                    end
+                 with
+                 | Some _ => fun f v => F (f v)
+                 | None => F
+                 end
+             | pattern.App f x
+               => @lift_with_bindings
+                   f _ _
+                   (@lift_with_bindings x _ _ F)
+             end.
+
+        Fixpoint app_pbase_type_interp_cps {T : Type} {K1 K2 : base.type -> Type}
+                 (F : forall t, K1 t -> K2 t -> T)
+                 {t}
+          : pbase_type_interp_cps qforall t K1
+            -> pbase_type_interp_cps qexists t K2 -> T
+          := match t return pbase_type_interp_cps qforall t K1
+                            -> pbase_type_interp_cps qexists t K2 -> T with
+             | pattern.base.type.any
+               => fun f tv => F _ (f _) (projT2 tv)
+             | pattern.base.type.type_base t
+               => fun f v => F _ f v
+             | pattern.base.type.prod A B
+               => @app_pbase_type_interp_cps
+                   _
+                   (fun A' => pbase_type_interp_cps qforall B (fun B' => K1 (A' * B')%etype))
+                   (fun A' => pbase_type_interp_cps qexists B (fun B' => K2 (A' * B')%etype))
+                   (fun A'
+                    => @app_pbase_type_interp_cps
+                        _
+                        (fun B' => K1 (A' * B')%etype)
+                        (fun B' => K2 (A' * B')%etype)
+                        (fun _ => F _)
+                        B)
+                   A
+             | pattern.base.type.list A
+               => @app_pbase_type_interp_cps T (fun A' => K1 (base.type.list A')) (fun A' => K2 (base.type.list A')) (fun _ => F _) A
+             end.
+
+        Fixpoint app_ptype_interp_cps {T : Type} {K1 K2 : type -> Type}
+                 (F : forall t, K1 t -> K2 t -> T)
+                 {t}
+          : ptype_interp_cps qforall t K1
+            -> ptype_interp_cps qexists t K2 -> T
+          := match t return ptype_interp_cps qforall t K1
+                            -> ptype_interp_cps qexists t K2 -> T with
+             | type.base t => app_pbase_type_interp_cps F
+             | type.arrow A B
+               => @app_ptype_interp_cps
+                   _
+                   (fun A' => ptype_interp_cps qforall B (fun B' => K1 (A' -> B')%etype))
+                   (fun A' => ptype_interp_cps qexists B (fun B' => K2 (A' -> B')%etype))
+                   (fun A'
+                    => @app_ptype_interp_cps
+                        _
+                        (fun B' => K1 (A' -> B')%etype)
+                        (fun B' => K2 (A' -> B')%etype)
+                        (fun _ => F _)
+                        B)
+                   A
+             end.
+
+        Fixpoint app_binding_data {T p} : forall (f : with_bindingsT p T) (v : binding_dataT p), T
+          := match p return forall (f : with_bindingsT p T) (v : binding_dataT p), T with
+             | pattern.Wildcard t
+               => app_ptype_interp_cps
+                   (K1:=fun t => value t -> T)
+                   (K2:=fun t => value t)
+                   (fun _ f v => f v)
+             | pattern.Ident idc
+               => match arg_types idc as ty
+                       return match ty with
+                              | Some t => t -> T
+                              | None => T
+                              end -> match ty return Type with
+                                    | Some t => t
+                                    | None => unit
+                                    end -> T
+                 with
+                 | Some t => fun f x => f x
+                 | None => fun v 'tt => v
+                 end
+             | pattern.App f x
+               => fun F '(vf, vx)
+                 => @app_binding_data _ x (@app_binding_data _ f F vf) vx
+             end.
+
+        (** XXX MOVEME? *)
+        Definition mkcast {P : type -> Type} {t1 t2 : type} : ~> (option (P t1 -> P t2))
+          := fun T k => type.try_make_transport_cps base.try_make_transport_cps P t1 t2 _ k.
+        Definition cast {P : type -> Type} {t1 t2 : type} (v : P t1) : ~> (option (P t2))
+          := fun T k => type.try_transport_cps base.try_make_transport_cps P t1 t2 v _ k.
+        Definition castb {P : base.type -> Type} {t1 t2 : base.type} (v : P t1) : ~> (option (P t2))
+          := fun T k => base.try_transport_cps P t1 t2 v _ k.
+        Definition castbe {t1 t2 : base.type} (v : expr t1) : ~> (option (expr t2))
+          := @castb expr t1 t2 v.
+        Definition castv {t1 t2} (v : value t1) : ~> (option (value t2))
+          := fun T k => type.try_transport_cps base.try_make_transport_cps value t1 t2 v _ k.
+           *)
+          Section with_do_again.
+            Context (dtree : @decision_tree pident)
+                    (rew1 : rewrite_rulesT1)
+                    (rew2 : rewrite_rulesT2)
+                    (Hrew : rewrite_rules_goodT rew1 rew2)
+                    (do_again1 : forall t : base.type, @expr.expr base.type ident (@value var1) t -> @UnderLets var1 (@expr var1 t))
+                    (do_again2 : forall t : base.type, @expr.expr base.type ident (@value var2) t -> @UnderLets var2 (@expr var2 t))
+                    (wf_do_again : forall G (t : base.type) e1 e2,
+                        expr.wf nil e1 e2
+                        -> UnderLets.wf (fun G' => expr.wf G') G (@do_again1 t e1) (@do_again2 t e2)).
+
+            Local Notation assemble_identifier_rewriters' var := (@assemble_identifier_rewriters' ident var pident full_types invert_bind_args type_of_pident pident_to_typed of_typed_ident arg_types bind_args try_make_transport_ident_cps dtree).
+            Local Notation assemble_identifier_rewriters var := (@assemble_identifier_rewriters ident var pident full_types invert_bind_args type_of_pident pident_to_typed eta_ident_cps of_typed_ident arg_types bind_args try_make_transport_ident_cps dtree).
+
+            Lemma wf_assemble_identifier_rewriters' G t re1 e1 re2 e2
+                  K1 K2
+                  (He : @wf_rawexpr G t re1 e1 re2 e2)
+                  (HK1 : forall P v, K1 P v = rew [P] (proj1 (eq_type_of_rawexpr_of_wf He)) in v)
+                  (HK2 : forall P v, K2 P v = rew [P] (proj2 (eq_type_of_rawexpr_of_wf He)) in v)
+              : wf_value_with_lets
+                  G
+                  (@assemble_identifier_rewriters' var1 rew1 do_again1 t re1 K1)
+                  (@assemble_identifier_rewriters' var2 rew2 do_again2 t re2 K2).
+            Proof.
+              revert dependent G; revert dependent re1; revert dependent re2; induction t as [t|s IHs d IHd];
+                intros; cbn [assemble_identifier_rewriters'].
+              { rewrite HK1, HK2; apply wf_eval_rewrite_rules; assumption. }
+              { hnf; intros; subst.
+                unshelve eapply IHd; cbn [type_of_rawexpr]; [ shelve | shelve | constructor | cbn; reflexivity | cbn; reflexivity ].
+                all: rewrite ?HK1, ?HK2.
+                { erewrite (proj1 (eq_expr_of_rawexpr_of_wf He)), (proj2 (eq_expr_of_rawexpr_of_wf He)).
+                  eapply wf_rawexpr_Proper_list; [ | eassumption ]; wf_t. }
+                { cbv [rValueOrExpr2]; break_innermost_match; constructor;
+                  try apply wf_reify;
+                  (eapply wf_value'_Proper_list; [ | eassumption ]); wf_t. } }
+            Qed.
+
+            Lemma wf_assemble_identifier_rewriters G t (idc : ident t)
+              : wf_value_with_lets
+                  G
+                  (@assemble_identifier_rewriters var1 rew1 do_again1 t idc)
+                  (@assemble_identifier_rewriters var2 rew2 do_again2 t idc).
+            Proof.
+              cbv [assemble_identifier_rewriters]; rewrite !eta_ident_cps_correct.
+              unshelve eapply wf_assemble_identifier_rewriters'; [ shelve | shelve | constructor | | ]; reflexivity.
+            Qed.
+          End with_do_again.
+        End with_var2.
+      End with_type.
+
+      Section full_with_var2.
+        Context {var1 var2 : type.type base.type -> Type}.
+        Local Notation expr := (@expr.expr base.type ident).
+        Local Notation value := (@Compile.value base.type ident).
+        Local Notation value_with_lets := (@Compile.value_with_lets base.type ident).
+        Local Notation UnderLets := (UnderLets.UnderLets base.type ident).
+        Local Notation reflect := (@Compile.reflect ident).
         Section with_rewrite_head.
-          Context (rewrite_head : forall t (idc : ident t), value_with_lets t).
+          Context (rewrite_head1 : forall t (idc : ident t), @value_with_lets var1 t)
+                  (rewrite_head2 : forall t (idc : ident t), @value_with_lets var2 t)
+                  (wf_rewrite_head : forall G t (idc1 idc2 : ident t),
+                      idc1 = idc2 -> wf_value_with_lets G (rewrite_head1 t idc1) (rewrite_head2 t idc2)).
 
+          Local Notation rewrite_bottomup1 := (@rewrite_bottomup var1 rewrite_head1).
+          Local Notation rewrite_bottomup2 := (@rewrite_bottomup var2 rewrite_head2).
+
+          Lemma wf_rewrite_bottomup G G' {t} e1 e2 (Hwf : expr.wf G e1 e2)
+                (HG : forall t v1 v2, List.In (existT _ t (v1, v2)) G -> wf_value G' v1 v2)
+            : wf_value_with_lets G' (@rewrite_bottomup1 t e1) (@rewrite_bottomup2 t e2).
+          Proof.
+            revert dependent G'; induction Hwf; intros; cbn [rewrite_bottomup].
+            all: repeat first [ reflexivity
+                              | solve [ eauto ]
+                              | apply wf_rewrite_head
+                              | apply wf_Base_value
+                              | apply wf_splice_value_with_lets
+                              | apply wf_splice_under_lets_with_value
+                              | apply wf_reify_and_let_binds_cps
+                              | apply UnderLets.wf_reify_and_let_binds_base_cps
+                              | apply wf_reflect
+                              | progress subst
+                              | progress destruct_head'_ex
+                              | progress cbv [wf_value_with_lets wf_value] in *
+                              | progress cbn [wf_value' fst snd] in *
+                              | progress intros
+                              | wf_safe_t_step
+                              | eapply wf_value'_Proper_list; [ | solve [ eauto ] ]
+                              | match goal with
+                                | [ |- UnderLets.wf _ _ _ _ ] => constructor
+                                | [ H : _ |- _ ] => apply H; clear H
+                                end ].
+          Qed.
         End with_rewrite_head.
 
-        Notation nbe := (@rewrite_bottomup (fun t idc => reflect (expr.Ident idc))).
+        Local Notation nbe var := (@rewrite_bottomup var (fun t idc => reflect (expr.Ident idc))).
 
-        Fixpoint repeat_rewrite
-                 (rewrite_head : forall (do_again : forall t : base.type, @expr value (type.base t) -> UnderLets (@expr var (type.base t)))
-                                            t (idc : ident t), value_with_lets t)
-                 (fuel : nat) {t} e : value_with_lets t
-          := @rewrite_bottomup
-               (rewrite_head
-                  (fun t' e'
-                   => match fuel with
-                      | Datatypes.O => nbe e'
-                      | Datatypes.S fuel' => @repeat_rewrite rewrite_head fuel' (type.base t') e'
-                      end%under_lets))
-               t e.
-
-        Definition rewrite rewrite_head fuel {t} e : expr t
-          := reify (@repeat_rewrite rewrite_head fuel t e).*)
-
-      End full.
-
-
-      About Rewrite.
-
-      Section all.
-        Import defaults.
-        Local Notation UnderLets := (UnderLets.UnderLets base.type ident).
-
-        Context (rewrite_head : forall var (do_again : forall t, @expr (@value _ ident var) (type.base t) -> UnderLets var (@expr var (type.base t))) t,
-                    ident t -> @value_with_lets _ ident var t).
-
-
-        (*
-        Lemma Wf_Rewrite fuel {t} (e : Expr t) (Hwf : Wf e) : Wf (Rewrite rewrite_head fuel e).
+        Lemma wf_nbe G G' {t} e1 e2
+              (Hwf : expr.wf G e1 e2)
+              (HG : forall t v1 v2, List.In (existT _ t (v1, v2)) G -> wf_value G' v1 v2)
+          : wf_value_with_lets G' (@nbe var1 t e1) (@nbe var2 t e2).
         Proof.
-          cbv [Rewrite]; intros ? ?.*)
-      End all.
+          eapply wf_rewrite_bottomup; try eassumption.
+          intros; subst; eapply wf_reflect; wf_t.
+        Qed.
+
+        Section with_rewrite_head2.
+          Context (rewrite_head1 : forall (do_again : forall t : base.type, @expr (@value var1) (type.base t) -> @UnderLets var1 (@expr var1 (type.base t)))
+                                          t (idc : ident t), @value_with_lets var1 t)
+                  (rewrite_head2 : forall (do_again : forall t : base.type, @expr (@value var2) (type.base t) -> @UnderLets var2 (@expr var2 (type.base t)))
+                                          t (idc : ident t), @value_with_lets var2 t)
+                  (wf_rewrite_head
+                   : forall
+                      do_again1
+                      do_again2
+                      (wf_do_again
+                       : forall G' G (t : base.type) e1 e2
+                                (HG : forall t v1 v2, List.In (existT _ t (v1, v2)) G -> wf_value G' v1 v2),
+                          expr.wf G e1 e2
+                          -> UnderLets.wf (fun G' => expr.wf G') G' (do_again1 t e1) (do_again2 t e2))
+                      G t (idc1 idc2 : ident t),
+                      idc1 = idc2 -> wf_value_with_lets G (rewrite_head1 do_again1 t idc1) (rewrite_head2 do_again2 t idc2)).
+
+          Lemma wf_repeat_rewrite fuel
+            : forall {t} G G' e1 e2
+                     (Hwf : expr.wf G e1 e2)
+                     (HG : forall t v1 v2, List.In (existT _ t (v1, v2)) G -> wf_value G' v1 v2),
+              wf_value_with_lets G' (@repeat_rewrite var1 rewrite_head1 fuel t e1) (@repeat_rewrite var2 rewrite_head2 fuel t e2).
+          Proof.
+            induction fuel as [|fuel IHfuel]; intros; cbn [repeat_rewrite]; eapply wf_rewrite_bottomup; try eassumption;
+              apply wf_rewrite_head; intros; [ eapply wf_nbe with (t:=type.base _) | eapply IHfuel with (t:=type.base _) ];
+                eassumption.
+          Qed.
+
+          Lemma wf_rewrite fuel
+            : forall {t} G G' e1 e2
+                     (Hwf : expr.wf G e1 e2)
+                     (HG : forall t v1 v2, List.In (existT _ t (v1, v2)) G -> wf_value G' v1 v2),
+              expr.wf G' (@rewrite var1 rewrite_head1 fuel t e1) (@rewrite var2 rewrite_head2 fuel t e2).
+          Proof. intros; eapply wf_reify, wf_repeat_rewrite; eassumption. Qed.
+        End with_rewrite_head2.
+      End full_with_var2.
+
+      Theorem Wf_Rewrite
+              (rewrite_head
+               : forall var
+                        (do_again : forall t : base.type, @expr (@value base.type ident var) (type.base t) -> @UnderLets.UnderLets base.type ident var (@expr var (type.base t)))
+                        t (idc : ident t), @value_with_lets base.type ident var t)
+              (wf_rewrite_head
+               : forall
+                  var1 var2
+                  do_again1
+                  do_again2
+                  (wf_do_again
+                   : forall (t : base.type) e1 e2,
+                      expr.wf nil e1 e2
+                      -> UnderLets.wf (fun G' => expr.wf G') nil (do_again1 t e1) (do_again2 t e2))
+                  t (idc : ident t),
+                  wf_value_with_lets nil (rewrite_head var1 do_again1 t idc) (rewrite_head var2 do_again2 t idc))
+              fuel {t} (e : Expr t) (Hwf : Wf e)
+        : Wf (@Rewrite rewrite_head fuel t e).
+      Proof.
+        intros var1 var2; cbv [Rewrite]; eapply wf_rewrite with (G:=nil); [ | apply Hwf | wf_t ].
+        intros; subst; eapply wf_value'_Proper_list; [ | eapply wf_rewrite_head ]; wf_t.
+        eapply wf_do_again; [ | eassumption ]; wf_t.
+      Qed.
     End Compile.
-    *)
 
     Lemma nbe_rewrite_head_eq : @nbe_rewrite_head = @nbe_rewrite_head0.
     Proof. reflexivity. Qed.
@@ -113,26 +1389,197 @@ Module Compilers.
     Lemma arith_all_rewrite_rules_eq : @arith_all_rewrite_rules = @arith_rewrite_rules.
     Proof. reflexivity. Qed.
 
+    Section good.
+      Context {var1 var2 : type -> Type}.
+
+      Local Notation rewrite_rules_goodT := (@Compile.rewrite_rules_goodT ident pattern.ident pattern.ident.arg_types var1 var2).
+
+      Lemma rlist_rect_cps_id {var} A P {ivar} N_case C_case ls T k
+        : @rlist_rect var A P ivar N_case C_case ls T k = k (@rlist_rect var A P ivar N_case C_case ls _ id).
+      Proof.
+        cbv [rlist_rect id Compile.option_bind']; rewrite !expr.reflect_list_cps_id.
+        destruct (invert_expr.reflect_list ls) eqn:?; cbn [Option.bind Option.sequence_return]; reflexivity.
+      Qed.
+      Lemma rlist_rect_cast_cps_id {var} A A' P {ivar} N_case C_case ls T k
+        : @rlist_rect_cast var A A' P ivar N_case C_case ls T k = k (@rlist_rect_cast var A A' P ivar N_case C_case ls _ id).
+      Proof.
+        cbv [rlist_rect_cast Compile.castbe Compile.castb id Compile.option_bind']; rewrite_type_transport_correct;
+          break_innermost_match; type_beq_to_eq; subst; cbn [eq_rect Option.bind Option.sequence_return]; [ | reflexivity ].
+        apply rlist_rect_cps_id.
+      Qed.
+
+      Local Ltac start_cps_id :=
+        lazymatch goal with
+        | [ |- In _ ?rewr -> _ ] => let h := head rewr in cbv [h]
+        end;
+        cbn [In combine]; intros; destruct_head'_or; inversion_sigma; subst; try reflexivity; destruct_head' False.
+
+      Local Ltac cps_id_step :=
+        first [ reflexivity
+              | progress destruct_head' False
+              | progress subst
+              | progress inversion_option
+              | progress cbv [id Compile.binding_dataT pattern.ident.arg_types Compile.ptype_interp Compile.ptype_interp_cps Compile.pbase_type_interp_cps Compile.value Compile.value' Compile.app_binding_data Compile.app_ptype_interp_cps Compile.app_pbase_type_interp_cps Compile.lift_with_bindings Compile.lift_ptype_interp_cps Compile.lift_pbase_type_interp_cps cpsbind cpscall cpsreturn cps_option_bind type_base rwhen] in *
+              | progress cbn [UnderLets.splice eq_rect projT1 projT2 Option.bind Option.sequence Option.sequence_return] in *
+              | progress type_beq_to_eq
+              | progress rewrite_type_transport_correct
+              | progress cbv [Compile.option_bind' Compile.castbe Compile.castb Compile.castv] in *
+              | progress break_innermost_match
+              | progress destruct_head'_sigT
+              | rewrite !expr.reflect_list_cps_id
+              | match goal with
+                | [ |- context[@rlist_rect_cast ?var ?A ?A' ?P ?ivar ?N_case ?C_case ?ls ?T ?k] ]
+                  => (tryif (let __ := constr:(eq_refl : k = (fun x => x)) in idtac)
+                       then fail
+                       else rewrite (@rlist_rect_cast_cps_id var A A' P ivar N_case C_case ls T k))
+                | [ |- context[@rlist_rect ?var ?A ?P ?ivar ?N_case ?C_case ?ls ?T ?k] ]
+                  => (tryif (let __ := constr:(eq_refl : k = (fun x => x)) in idtac)
+                       then fail
+                       else rewrite (@rlist_rect_cps_id var A P ivar N_case C_case ls T k))
+                end
+              | progress cbv [Option.bind] in *
+              | break_match_step ltac:(fun _ => idtac) ].
+
+      Local Ltac cps_id_t := start_cps_id; repeat cps_id_step.
+
+      Lemma nbe_cps_id {var} p r
+        : In (existT _ p r) (@nbe_rewrite_rules var)
+          -> forall v T k, r v T k = k (r v _ id).
+      Proof. cps_id_t. Qed.
+
+      Lemma arith_cps_id max_const {var} p r
+        : In (existT _ p r) (@arith_rewrite_rules var max_const)
+          -> forall v T k, r v T k = k (r v _ id).
+      Proof. cps_id_t. Qed.
+
+      Lemma fancy_cps_id invert_low invert_high {var} p r
+        : In (existT _ p r) (@fancy_rewrite_rules var invert_low invert_high)
+          -> forall v T k, r v T k = k (r v _ id).
+      Proof. cps_id_t. Qed.
+
+      Local Ltac start_good cps_id rewrite_rules :=
+        split; [ reflexivity | ];
+          repeat apply conj; try solve [ eapply cps_id ]; [];
+            cbv [rewrite_rules]; cbn [In combine];
+              intros; destruct_head'_or; inversion_prod; inversion_sigma; subst; destruct_head' False;
+              (split; [ reflexivity | ]).
+
+      Local Ltac good_t_step :=
+        first [ progress subst
+              | progress cbv [id Compile.binding_dataT pattern.ident.arg_types Compile.ptype_interp Compile.ptype_interp_cps Compile.pbase_type_interp_cps Compile.value Compile.value' Compile.app_binding_data Compile.app_ptype_interp_cps Compile.app_pbase_type_interp_cps Compile.lift_with_bindings Compile.lift_ptype_interp_cps Compile.lift_pbase_type_interp_cps cpsbind cpscall cpsreturn cps_option_bind type_base Compile.wf_binding_dataT Compile.wf_ptype_interp_id Compile.wf_ptype_interp_cps Compile.wf_pbase_type_interp_cps ident.smart_Literal rwhen AnyExpr.unwrap] in *
+              | progress destruct_head'_sig
+              | progress cbn [eq_rect option_eq projT1 projT2 fst snd base.interp In combine Option.bind Option.sequence Option.sequence_return UnderLets.splice] in *
+              | progress destruct_head'_prod
+              | progress destruct_head'_sigT
+              | progress intros
+              | progress eliminate_hprop_eq
+              | progress cbv [Compile.option_bind' Compile.castbe Compile.castb Compile.castv] in *
+              | progress type_beq_to_eq
+              | progress rewrite_type_transport_correct
+              | break_innermost_match_step
+              | wf_safe_t_step
+              | rewrite !expr.reflect_list_cps_id
+              | congruence
+              | match goal with
+                | [ |- expr.wf _ (reify_list _) (reify_list _) ] => rewrite expr.wf_reify_list
+                | [ |- context[length ?ls] ] => tryif is_var ls then fail else (progress autorewrite with distr_length)
+                | [ |- ex _ ] => eexists
+                | [ |- UnderLets.wf _ _ _ _ ] => constructor
+                | [ |- UnderLets.wf _ _ (UnderLets.splice _ _) (UnderLets.splice _ _) ] => eapply UnderLets.wf_splice
+                | [ |- Compile.wf_anyexpr _ _ _ _ ] => constructor
+                | [ H : Compile.wf_value ?G ?e1 ?e2 |- UnderLets.wf _ ?G (?e1 _) (?e2 _) ] => eapply (H nil)
+                | [ H : Compile.wf_value ?G ?e1 ?e2 |- UnderLets.wf _ ?G (?e1 _ _) (?e2 _ _) ]
+                  => eapply UnderLets.wf_Proper_list; [ | | eapply H; [ reflexivity | | reflexivity | ] ]; revgoals
+                | [ |- context[@rlist_rect_cast ?var ?A ?A' ?P ?ivar ?N_case ?C_case ?ls ?T ?k] ]
+                  => (tryif (let __ := constr:(eq_refl : k = (fun x => x)) in idtac)
+                       then fail
+                       else rewrite (@rlist_rect_cast_cps_id var A A' P ivar N_case C_case ls T k))
+                | [ |- context[@rlist_rect ?var ?A ?P ?ivar ?N_case ?C_case ?ls ?T ?k] ]
+                  => (tryif (let __ := constr:(eq_refl : k = (fun x => x)) in idtac)
+                       then fail
+                       else rewrite (@rlist_rect_cps_id var A P ivar N_case C_case ls T k))
+                | [ |- ?x = ?x /\ _ ] => split; [ reflexivity | ]
+                end
+              | solve [ wf_t ]
+(*| progress cbv [Option.bind]
+                          | break_match_step ltac:(fun _ => idtac)*) ].
+
+      Lemma nbe_rewrite_rules_good
+        : rewrite_rules_goodT nbe_rewrite_rules nbe_rewrite_rules.
+      Proof.
+        start_good (@nbe_cps_id) (@nbe_rewrite_rules).
+        all: repeat good_t_step.
+      Admitted.
+
+      Lemma arith_rewrite_rules_good max_const
+        : rewrite_rules_goodT (arith_rewrite_rules max_const) (arith_rewrite_rules max_const).
+      Proof.
+        start_good (@arith_cps_id) (@arith_rewrite_rules).
+        all: repeat good_t_step.
+      Admitted.
+
+      Lemma fancy_rewrite_rules_good
+            (invert_low invert_high : Z -> Z -> option Z)
+            (Hlow : forall s v v', invert_low s v = Some v' -> v = Z.land v' (2^(s/2)-1))
+            (Hhigh : forall s v v', invert_high s v = Some v' -> v = Z.shiftr v' (s/2))
+        : rewrite_rules_goodT (fancy_rewrite_rules invert_low invert_high) (fancy_rewrite_rules invert_low invert_high).
+      Proof.
+        start_good (@fancy_cps_id) (@fancy_rewrite_rules).
+        all: repeat good_t_step.
+        all: cbv [Option.bind].
+        all: repeat good_t_step.
+      Qed.
+    End good.
+
+    Local Ltac start_Wf_or_interp_proof rewrite_head_eq all_rewrite_rules_eq rewrite_head0 :=
+      let Rewrite := lazymatch goal with
+                     | [ |- Wf ?e ] => head e
+                     | [ |- Interp ?e == _ ] => head e
+                     end in
+      cbv [Rewrite]; rewrite rewrite_head_eq; cbv [rewrite_head0]; rewrite all_rewrite_rules_eq.
+    Local Ltac start_Wf_proof rewrite_head_eq all_rewrite_rules_eq rewrite_head0 :=
+      start_Wf_or_interp_proof rewrite_head_eq all_rewrite_rules_eq rewrite_head0;
+      apply Compile.Wf_Rewrite; [ | assumption ];
+      let wf_do_again := fresh "wf_do_again" in
+      (intros ? ? ? ? wf_do_again ? ?);
+      eapply @Compile.wf_assemble_identifier_rewriters;
+      eauto using
+            pattern.ident.to_typed_invert_bind_args,
+      pattern.ident.ident_beq,
+      pattern.ident.internal_ident_dec_bl,
+      pattern.ident.try_make_transport_ident_cps_correct,
+      pattern.ident.eta_ident_cps_correct
+        with nocore;
+      [ .. | intros; eapply UnderLets.wf_Proper_list; [ | | eapply wf_do_again; assumption ]; solve [ wf_t ] ].
+    Local Ltac start_Interp_proof rewrite_head_eq all_rewrite_rules_eq rewrite_head0 :=
+      start_Wf_or_interp_proof rewrite_head_eq all_rewrite_rules_eq rewrite_head0.
+
     Lemma Wf_RewriteNBE {t} e (Hwf : Wf e) : Wf (@RewriteNBE t e).
     Proof.
-      cbv [RewriteNBE]; rewrite nbe_rewrite_head_eq; cbv [nbe_rewrite_head0]; rewrite nbe_all_rewrite_rules_eq.
-    Admitted.
+      start_Wf_proof nbe_rewrite_head_eq nbe_all_rewrite_rules_eq (@nbe_rewrite_head0).
+      apply nbe_rewrite_rules_good.
+    Qed.
     Lemma Wf_RewriteArith (max_const_val : Z) {t} e (Hwf : Wf e) : Wf (@RewriteArith max_const_val t e).
     Proof.
-      cbv [RewriteArith]; rewrite arith_rewrite_head_eq; cbv [arith_rewrite_head0]; rewrite arith_all_rewrite_rules_eq.
-    Admitted.
-    Lemma Wf_RewriteToFancy (invert_low invert_high : Z -> Z -> option Z) {t} e (Hwf : Wf e) : Wf (@RewriteToFancy invert_low invert_high t e).
+      start_Wf_proof arith_rewrite_head_eq arith_all_rewrite_rules_eq (@arith_rewrite_head0).
+      apply arith_rewrite_rules_good.
+    Qed.
+    Lemma Wf_RewriteToFancy (invert_low invert_high : Z -> Z -> option Z)
+            (Hlow : forall s v v', invert_low s v = Some v' -> v = Z.land v' (2^(s/2)-1))
+            (Hhigh : forall s v v', invert_high s v = Some v' -> v = Z.shiftr v' (s/2))
+            {t} e (Hwf : Wf e) : Wf (@RewriteToFancy invert_low invert_high t e).
     Proof.
-      cbv [RewriteToFancy]; rewrite fancy_rewrite_head_eq; cbv [fancy_rewrite_head0]; rewrite fancy_all_rewrite_rules_eq.
-    Admitted.
+      start_Wf_proof fancy_rewrite_head_eq fancy_all_rewrite_rules_eq (@fancy_rewrite_head0).
+      apply fancy_rewrite_rules_good; assumption.
+    Qed.
 
     Lemma Interp_RewriteNBE {t} e (Hwf : Wf e) : Interp (@RewriteNBE t e) == Interp e.
     Proof.
-      cbv [RewriteNBE]; rewrite nbe_rewrite_head_eq; cbv [nbe_rewrite_head0]; rewrite nbe_all_rewrite_rules_eq.
+      start_Interp_proof nbe_rewrite_head_eq nbe_all_rewrite_rules_eq (@nbe_rewrite_head0).
     Admitted.
     Lemma Interp_RewriteArith (max_const_val : Z) {t} e (Hwf : Wf e) : Interp (@RewriteArith max_const_val t e) == Interp e.
     Proof.
-      cbv [RewriteArith]; rewrite arith_rewrite_head_eq; cbv [arith_rewrite_head0]; rewrite arith_all_rewrite_rules_eq.
+      start_Interp_proof arith_rewrite_head_eq arith_all_rewrite_rules_eq (@arith_rewrite_head0).
     Admitted.
 
     Lemma Interp_RewriteToFancy (invert_low invert_high : Z -> Z -> option Z)
@@ -141,7 +1588,7 @@ Module Compilers.
           {t} e (Hwf : Wf e)
       : Interp (@RewriteToFancy invert_low invert_high t e) == Interp e.
     Proof.
-      cbv [RewriteToFancy]; rewrite fancy_rewrite_head_eq; cbv [fancy_rewrite_head0]; rewrite fancy_all_rewrite_rules_eq.
+      start_Interp_proof fancy_rewrite_head_eq fancy_all_rewrite_rules_eq (@fancy_rewrite_head0).
     Admitted.
   End RewriteRules.
 
